@prefix inspire-concept: <http://bp4mc2.org/inspire/id/concept/>.
@prefix inspire-collection: <http://bp4mc2.org/inspire/id/collection/>.
@prefix inspire-scheme: <http://bp4mc2.org/inspire/id/conceptscheme/>.
@prefix inspire-shape: <http://bp4mc2.org/inspire/def/inspire/>.
@prefix inspire-lex: <http://bp4mc2.org/inspire/id/regelgeving/>.
@prefix inspire: <http://bp4mc2.org/inspire/def/inspire#>.
@prefix inspire-meta: <http://bp4mc2.org/inspire/def/meta#>.

@prefix adms: <http://www.w3.org/ns/adms#> .
@prefix dash: <http://datashapes.org/dash#> .
@prefix dc: <http://purl.org/dc/elements/1.1/> .
@prefix dcat: <http://www.w3.org/ns/dcat#> .
@prefix dct: <http://purl.org/dc/terms/> .
@prefix dctype: <http://purl.org/dc/dcmitype/>.
@prefix foaf: <http://xmlns.com/foaf/0.1/> .
@prefix org: <http://www.w3.org/ns/org#> .
@prefix owl: <http://www.w3.org/2002/07/owl#> .
@prefix prov: <http://www.w3.org/ns/prov#> .
@prefix rdf: <http://www.w3.org/1999/02/22-rdf-syntax-ns#> .
@prefix rdfs: <http://www.w3.org/2000/01/rdf-schema#> .
@prefix schema: <http://schema.org/> .
@prefix sh: <http://www.w3.org/ns/shacl#> .
@prefix skos: <http://www.w3.org/2004/02/skos/core#> .
@prefix skosxl: <http://www.w3.org/2008/05/skos-xl#> .
@prefix spdx: <http://spdx.org/rdf/terms#> .
@prefix tosh: <http://topbraid.org/tosh#> .
@prefix vcard: <http://www.w3.org/2006/vcard/ns#> .
@prefix xml: <http://www.w3.org/XML/1998/namespace> .
@prefix xsd: <http://www.w3.org/2001/XMLSchema#> .
@prefix frbr: <http://purl.org/vocab/frbr/core#>.

# ============================
# Metadata originele wetgeving
# ============================

#
# INSPIRE Directive
#
inspire-lex:Directive2007-2 a frbr:Work;
  rdfs:label "The INSPIRE directive"@en;
  foaf:isPrimaryTopicOf <http://data.europa.eu/eli/dir/2007/2>
.
inspire-lex:Directive2007-2-0 a frbr:Expression;
  rdfs:label "The INSPIRE directive"@en;
  foaf:isPrimaryTopicOf <http://eur-lex.europa.eu/legal-content/EN/ALL/?uri=CELEX:32007L0002>
.
inspire-lex:Article13-1-a a frbr:Work;
  rdfs:label "Article 13 clause 1.a";
  dct:isPartOf inspire-lex:Directive2007-2
.

#
# INSPIRE regulation for metadata
#
inspire-lex:Regulation2008-1205 a frbr:Work;
  rdfs:label "INSPIRE regulation for metadata"@en;
  foaf:isPrimaryTopicOf <http://eur-lex.europa.eu/eli/reg/2008/1205>
.
inspire-lex:Regulation2008-1205 a frbr:Expression;
  rdfs:label "INSPIRE regulation for metadata"@en;
  foaf:isPrimaryTopicOf <http://eur-lex.europa.eu/legal-content/EN/ALL/?uri=CELEX:32008R1205>
.
inspire-lex:Regulation2008-1205a a frbr:Expression;
  rdfs:label "Correction of INSPIRE regulation for metadata"@en;
  foaf:isPrimaryTopicOf <http://eur-lex.europa.eu/legal-content/EN/ALL/?uri=CELEX:32008R1205R(02)>;
  inspire-meta:isCorrectionOf inspire-lex:Regulation2008-1205
.
# Parts
inspire-lex:PartA a frbr:Work;
  rdfs:label "Part A"@en;
  dct:isPartOf inspire-lex:Regulation2008-1205
.
inspire-lex:PartB a frbr:Work;
  rdfs:label "Part B"@en;
  dct:isPartOf inspire-lex:Regulation2008-1205
.
inspire-lex:PartA1 a frbr:Work;
  rdfs:label "Part A 1"@en;
  rdfs:label "Deel A 1"@nl;
  dct:isPartOf inspire-lex:PartA
.
inspire-lex:PartA2 a frbr:Work;
  rdfs:label "Part A 2"@en;
  rdfs:label "Deel A 2"@nl;
  dct:isPartOf inspire-lex:PartA
.
inspire-lex:PartB01-1 a frbr:Work;
  rdfs:label "Part B 1.1"@en;
  rdfs:label "Deel B 1.1"@nl;
  dct:isPartOf inspire-lex:PartB
.
inspire-lex:PartB01-2 a frbr:Work;
  rdfs:label "Part B 1.2"@en;
  dct:isPartOf inspire-lex:PartB
.
inspire-lex:PartB01-3 a frbr:Work;
  rdfs:label "Part B 1.3"@en;
  dct:isPartOf inspire-lex:PartB
.
inspire-lex:PartB01-4 a frbr:Work;
  rdfs:label "Part B 1.4"@en;
  dct:isPartOf inspire-lex:PartB
.
inspire-lex:PartB01-5 a frbr:Work;
  rdfs:label "Part B 1.5"@en;
  dct:isPartOf inspire-lex:PartB
.
inspire-lex:PartB01-6 a frbr:Work;
  rdfs:label "Part B 1.6"@en;
  dct:isPartOf inspire-lex:PartB
.
inspire-lex:PartB01-7 a frbr:Work;
  rdfs:label "Part B 1.7"@en;
  dct:isPartOf inspire-lex:PartB
.
inspire-lex:PartB02-1 a frbr:Work;
  rdfs:label "Part B 2.1"@en;
  dct:isPartOf inspire-lex:PartB
.
inspire-lex:PartB02-2 a frbr:Work;
  rdfs:label "Part B 2.2"@en;
  dct:isPartOf inspire-lex:PartB
.
inspire-lex:PartB03 a frbr:Work;
  rdfs:label "Part B 3"@en;
  dct:isPartOf inspire-lex:PartB
.
inspire-lex:PartB03-1 a frbr:Work;
  rdfs:label "Part B 3.1"@en;
  dct:isPartOf inspire-lex:PartB03
.
inspire-lex:PartB03-2 a frbr:Work;
  rdfs:label "Part B 3.2"@en;
  dct:isPartOf inspire-lex:PartB03
.
inspire-lex:PartB04-1 a frbr:Work;
  rdfs:label "Part B 4.1"@en;
  dct:isPartOf inspire-lex:PartB
.
inspire-lex:PartB05 a frbr:Work;
  rdfs:label "Part B 5"@en;
  dct:isPartOf inspire-lex:PartB
.
inspire-lex:PartB05-1 a frbr:Work;
  rdfs:label "Part B 5.1"@en;
  dct:isPartOf inspire-lex:PartB05
.
inspire-lex:PartB05-2 a frbr:Work;
  rdfs:label "Part B 5.2"@en;
  dct:isPartOf inspire-lex:PartB05
.
inspire-lex:PartB05-3 a frbr:Work;
  rdfs:label "Part B 5.3"@en;
  dct:isPartOf inspire-lex:PartB05
.
inspire-lex:PartB05-4 a frbr:Work;
  rdfs:label "Part B 5.4"@en;
  dct:isPartOf inspire-lex:PartB05
.
inspire-lex:PartB06-1 a frbr:Work;
  rdfs:label "Part B 6.1"@en;
  dct:isPartOf inspire-lex:PartB
.
inspire-lex:PartB06-2 a frbr:Work;
  rdfs:label "Part B 6.2"@en;
  dct:isPartOf inspire-lex:PartB
.
inspire-lex:PartB07 a frbr:Work;
  rdfs:label "Part B 7"@en;
  dct:isPartOf inspire-lex:PartB
.
inspire-lex:PartB07-1 a frbr:Work;
  rdfs:label "Part B 7.1"@en;
  dct:isPartOf inspire-lex:PartB07
.
inspire-lex:PartB07-2 a frbr:Work;
  rdfs:label "Part B 7.2"@en;
  dct:isPartOf inspire-lex:PartB07
.
inspire-lex:PartB08-1 a frbr:Work;
  rdfs:label "Part B 8.1"@en;
  dct:isPartOf inspire-lex:PartB
.
inspire-lex:PartB08-2 a frbr:Work;
  rdfs:label "Part B 8.2"@en;
  dct:isPartOf inspire-lex:PartB
.
inspire-lex:PartB09 a frbr:Work;
  rdfs:label "Part B 9"@en;
  dct:isPartOf inspire-lex:PartB
.
inspire-lex:PartB09-1 a frbr:Work;
  rdfs:label "Part B 9.1"@en;
  dct:isPartOf inspire-lex:PartB09
.
inspire-lex:PartB09-2 a frbr:Work;
  rdfs:label "Part B 9.2"@en;
  dct:isPartOf inspire-lex:PartB09
.
inspire-lex:PartB10-1 a frbr:Work;
  rdfs:label "Part B 10.1"@en;
  dct:isPartOf inspire-lex:PartB
.
inspire-lex:PartB10-2 a frbr:Work;
  rdfs:label "Part B 10.2"@en;
  dct:isPartOf inspire-lex:PartB
.
inspire-lex:PartB10-3 a frbr:Work;
  rdfs:label "Part B 10.3"@en;
  dct:isPartOf inspire-lex:PartB
.

#
# INSPIRE regulation for interoperability of spatial data sets and services
#
inspire-lex:Regulation2010-1089 a frbr:Work;
  rdfs:label "INSPIRE regulation for interoperability of spatial data sets and services"@en;
  foaf:isPrimaryTopicOf <http://eur-lex.europa.eu/eli/reg/2010/1089>
.
inspire-lex:Regulation2010-1089-0 a frbr:Expression;
  rdfs:label "INSPIRE regulation for interoperability of spatial data sets and services"@en;
  foaf:isPrimaryTopicOf <http://eur-lex.europa.eu/legal-content/EN/ALL/?uri=CELEX:32010R1089>
.
inspire-lex:Regulation2010-1089-1 a frbr:Expression;
  rdfs:label "First ammendment of INSPIRE regulation for interoperability of spatial data sets and services"@en;
  foaf:isPrimaryTopicOf <http://eur-lex.europa.eu/legal-content/EN/ALL/?uri=CELEX:32011R0102>
.
inspire-lex:Regulation2010-1089-2 a frbr:Expression;
  rdfs:label "Second ammendment of INSPIRE regulation for interoperability of spatial data sets and services"@en;
  foaf:isPrimaryTopicOf <http://eur-lex.europa.eu/legal-content/EN/ALL/?uri=CELEX:32013R1253>
.
inspire-lex:Regulation2010-1089-3 a frbr:Expression;
  rdfs:label "Third ammendment of INSPIRE regulation for interoperability of spatial data sets and services"@en;
  foaf:isPrimaryTopicOf <http://eur-lex.europa.eu/legal-content/EN/ALL/?uri=CELEX:32014R1312>
.
# Parts
inspire-lex:Article02 a frbr:Work;
  rdfs:label "Article 2"@en;
  dct:isPartOf inspire-lex:Regulation2010-1089
.
inspire-lex:Article02-05 a frbr:Work;
  rdfs:label "Article 2 clause 5"@en;
  dct:isPartOf inspire-lex:Article02
.
inspire-lex:Article02-07 a frbr:Work;
  rdfs:label "Article 2 clause 7"@en;
  dct:isPartOf inspire-lex:Article02
.
inspire-lex:Article02-31 a frbr:Work;
  rdfs:label "Article 2 clause 31"@en;
  dct:isPartOf inspire-lex:Article02
.
inspire-lex:Article02-32 a frbr:Work;
  rdfs:label "Article 2 clause 32"@en;
  dct:isPartOf inspire-lex:Article02
.
inspire-lex:Article13-1 a frbr:Work;
  rdfs:label "Article 13 clause 1"@en;
  dct:isPartOf inspire-lex:Regulation2010-1089
.
inspire-lex:Article13-2 a frbr:Work;
  rdfs:label "Article 13 clause 2"@en;
  dct:isPartOf inspire-lex:Regulation2010-1089
.
inspire-lex:Article13-3 a frbr:Work;
  rdfs:label "Article 13 clause 3"@en;
  dct:isPartOf inspire-lex:Regulation2010-1089
.
inspire-lex:Article13-4 a frbr:Work;
  rdfs:label "Article 13 clause 4"@en;
  dct:isPartOf inspire-lex:Regulation2010-1089
.
inspire-lex:Article13-5 a frbr:Work;
  rdfs:label "Article 13 clause 5"@en;
  dct:isPartOf inspire-lex:Regulation2010-1089
.
inspire-lex:Article13-6 a frbr:Work;
  rdfs:label "Article 13 clause 6"@en;
  dct:isPartOf inspire-lex:Regulation2010-1089
.
inspire-lex:AnnexVPartB1 a frbr:Work;
  rdfs:label "Annex V Part B.1 (annex of Article 14a)"@en;
  dct:isPartOf inspire-lex:Regulation2010-1089
.
inspire-lex:AnnexVIPartB3 a frbr:Work;
  rdfs:label "Annex VI Part B.3 (annex of Article 14b)"@en;
  dct:isPartOf inspire-lex:Regulation2010-1089
.
inspire-lex:AnnexVIPartB4 a frbr:Work;
  rdfs:label "Annex VI Part B.4 (annex of Article 14b)"@en;
  dct:isPartOf inspire-lex:Regulation2010-1089
.
inspire-lex:AnnexVIPartB4-1 a frbr:Work;
  rdfs:label "Annex VI Part B.4.1 (annex of Article 14b)"@en;
  dct:isPartOf inspire-lex:AnnexVIPartB4
.
inspire-lex:AnnexVIPartB4-1-1 a frbr:Work;
  rdfs:label "Annex VI Part B.4.1.1 (annex of Article 14b)"@en;
  dct:isPartOf inspire-lex:AnnexVIPartB4-1
.
inspire-lex:AnnexVIPartB4-1-2 a frbr:Work;
  rdfs:label "Annex VI Part B.4.1.2 (annex of Article 14b)"@en;
  dct:isPartOf inspire-lex:AnnexVIPartB4-1
.
inspire-lex:AnnexVIPartB4-1-3 a frbr:Work;
  rdfs:label "Annex VI Part B.4.1.3 (annex of Article 14b)"@en;
  dct:isPartOf inspire-lex:AnnexVIPartB4-1
.
inspire-lex:AnnexVIPartB4-2-1 a frbr:Work;
  rdfs:label "Annex VI Part B.4.2.1 (annex of Article 14b)"@en;
  dct:isPartOf inspire-lex:AnnexVIPartB4
.
inspire-lex:AnnexVIPartB4-2-2 a frbr:Work;
  rdfs:label "Annex VI Part B.4.2.2 (annex of Article 14b)"@en;
  dct:isPartOf inspire-lex:AnnexVIPartB4
.
inspire-lex:AnnexVIPartB4-2-3 a frbr:Work;
  rdfs:label "Annex VI Part B.4.2.3 (annex of Article 14b)"@en;
  dct:isPartOf inspire-lex:AnnexVIPartB4
.
inspire-lex:AnnexVIIPartB3 a frbr:Work;
  rdfs:label "Annex VII Part B.3 (annex of Article 14b)"@en;
  dct:isPartOf inspire-lex:Regulation2010-1089
.

# =================================
# Begrippen uit originele wetgeving
# =================================
inspire-scheme:Inspire a skos:ConceptScheme;
  rdfs:label "Inspire"@en;
.
#
# Part A
#
inspire-concept:Resource a skos:Concept;
  dct:source inspire-lex:PartA1;
  rdfs:label "Resource"@en;
  rdfs:label "Bron"@nl;
  skos:definition "An information resource that has a direct or indirect reference to a specific location or geographic area."@en;
  skos:definition "een informatiebron die een directe of indirecte verwijzing bevat naar een specifieke plaats of geografisch gebied"@nl;
. 
#
# Part B
#
inspire-concept:ResourceTitle a skos:Concept;
  dct:source inspire-lex:PartB01-1;
  rdfs:label "Resource title"@en;
  rdfs:label "Titel van de bron"@nl;
  skos:definition "This a characteristic, and often unique, name by which the resource is known."@en;
  skos:definition "Dit is een kenmerkende en vaak unieke naam waaronder de bron bekend staat.";
  skos:scopeNote "The value domain of this metadata element is free text."@en;
  skos:scopeNote "Het waardedomein van dit metagegevenselement is vrije tekst.";
.
inspire-concept:ResourceAbstract a skos:Concept;
  dct:source inspire-lex:PartB01-2;
  rdfs:label "Resource abstract"@en;
  rdfs:label "Samenvatting van de bron"@nl;
  skos:definition "This is a brief narrative summary of the content of the resource."@en;
  skos:scopeNote "The value domain of this metadata element is free text.";
.
inspire-concept:ResourceType a skos:Concept;
  dct:source inspire-lex:PartB01-3;
  rdfs:label "Resource type"@en;
  rdfs:label "Type bron"@nl;
  skos:definition "This is the type of resource being described by the metadata."@en;
  skos:scopeNote "The value domain of this metadata element is defined in Part D.1.";
.
inspire-concept:ResourceLocator a skos:Concept;
  dct:source inspire-lex:PartB01-4;
  rdfs:label "Resource locator"@en;
  rdfs:label "Resource locator"@nl;
  skos:definition "The resource locator defines the link(s) to the resource and/or the link to additional information about the resource."@en;
  skos:scopeNote "The value domain of this metadata element is a character string, commonly expressed as uniform resource locator (URL)."@en;
.
inspire-concept:UniqueResourceIdentifier a skos:Concept;
  dct:source inspire-lex:PartB01-5;
  rdfs:label "Unique resource identifier"@en;
  rdfs:label "Unieke identifier van de bron"@nl;
  skos:definition "A value uniquely identifying the resource."@en;
  skos:scopeNote "The value domain of this metadata element is a mandatory character string code, generally assigned by the data owner, and a character string namespace uniquely identifying the context of the identifier code (for example, the data owner)."@en;
.
inspire-concept:CoupledResource a skos:Concept;
  dct:source inspire-lex:PartB01-6;
  rdfs:label "Coupled resource"@en;
  rdfs:label "Coupled resource"@nl;
  skos:definition "If the resource is a spatial data service, this metadata element identifies, where relevant, the target spatial data set(s) of the service through their unique resource identifiers (URI)."@en;
  skos:scopeNote "The value domain of this metadata element is a mandatory character string code, generally assigned by the data owner, and a character string namespace uniquely identifying the context of the identifier code (for example, the data owner)."@en;
.
inspire-concept:ResourceLanguage a skos:Concept;
  dct:source inspire-lex:PartB01-7;
  rdfs:label "Resource language"@en;
  rdfs:label "Taal van de bron"@nl;
  skos:definition "The language(s) used within the resource."@en;
  skos:scopeNote "The value domain of this metadata element is limited to the languages defined in ISO 639-2."@en;
.
inspire-concept:TopicCategory a skos:Concept;
  dct:source inspire-lex:PartB02-1;
  rdfs:label "Topic category"@en;
  rdfs:label "Onderwerpcategorie"@nl;
  skos:definition "The topic category is a high-level classification scheme to assist in the grouping and topic-based search of available spatial data resources."@en;
  skos:scopeNote "The value domain of this metadata element is defined in Part D.2.";
.
inspire-concept:SpatialDataServiceType a skos:Concept;
  dct:source inspire-lex:PartB02-2;
  rdfs:label "Spatial data service type"@en;
  rdfs:label "Type dienst met betrekking tot ruimtelijke gegevens"@nl;
  skos:definition "This is a classification to assist in the search of available spatial data services. A specific service shall be categorised in only one category."@en;
  skos:scopeNote "The value domain of this metadata element is defined in Part D.3."@en;
.
inspire-concept:Keyword a skos:Concept;
  dct:source inspire-lex:PartB03;
  rdfs:label "Keyword"@en;
  rdfs:label "Trefwoord"@nl;
  skos:definition "For each keyword, the following metadata elements shall be provided: [section 3.1 and 3.2]"@en;
  skos:scopeNote "If the resource is a spatial data service, at least one keyword from Part D.4 shall be provided."@en;
  skos:scopeNote "If a resource is a spatial data set or spatial data set series, at least one keyword shall be provided from the general environmental multilingual thesaurus (GEMET) describing the relevant spatial data theme as defined in Annex I, II or III to Directive 2007/2/EC."@en;
.
inspire-concept:KeywordValue a skos:Concept;
  dct:source inspire-lex:PartB03-1;
  rdfs:label "Keyword value"@en;
  rdfs:label "Trefwoordwaarde"@nl;
  skos:definition "The keyword value is a commonly used word, formalised word or phrase used to describe the subject. While the topic category is too coarse for detailed queries, keywords help narrowing a full text search and they allow for structured keyword search."@en;
  skos:scopeNote "The value domain of this metadata element is free text."@en;
.
inspire-concept:KeywordOriginatingControlledVocabulary a skos:Concept;
  dct:source inspire-lex:PartB03-2;
  rdfs:label "Keyword originating controlled vocabulary"@en;
  rdfs:label "Origineel gecontroleerd vocabulaire van het trefwoord"@nl;
  skos:definition "If the keyword value originates from a controlled vocabulary (thesaurus, ontology), for example GEMET, the citation of the originating controlled vocabulary shall be provided."@en;
  skos:scopeNote "This citation shall include at least the title and a reference date (date of publication, date of last revision or of creation) of the originating controlled vocabulary."@en;
.
inspire-concept:GeographicBoundingBox a skos:Concept;
  dct:source inspire-lex:PartB04-1;
  rdfs:label "Geographic bounding box"@en;
  rdfs:label "Geografische rechthoek"@nl;
  skos:definition "This is the extent of the resource in the geographic space, given as a bounding box."@en;
  skos:scopeNote "The bounding box shall be expressed with westbound and eastbound longitudes, and southbound and northbound latitudes in decimal degrees, with a precision of at least two decimals."@en;
.
inspire-concept:TemporalReference a skos:Concept;
  dct:source inspire-lex:PartB05;
  rdfs:label "Temporal reference"@en;
  rdfs:label "Tijdsreferentie"@nl;
  skos:definition "This metadata element addresses the requirement to have information on the temporal dimension of the data as referred to in Article 8(2)(d) of Directive 2007/2/EC. At least one of the metadata elements referred to in points 5.1 to 5.4 shall be provided."@en;
  skos:scopeNote "The value domain of the metadata elements referred to in points 5.1 to 5.4 is a set of dates. Each date shall refer to a temporal reference system and shall be expressed in a form compatible with that system. The default reference system shall be the Gregorian calendar, with dates expressed in accordance with ISO 8601."@en;
.
inspire-concept:TemporalExtent a skos:Concept;
  dct:source inspire-lex:PartB05-1;
  rdfs:label "Temporal extent"@en;
  rdfs:label "Temporele dekking"@nl;
  skos:definition "The temporal extent defines the time period covered by the content of the resource."@en;
  skos:scopeNote "This time period may be expressed as any of the following: (a) an individual date, (b) an interval of dates expressed through the starting date and end date of the interval, (c) a mix of individual dates and intervals of dates."@en;
.
inspire-concept:DateOfPublication a skos:Concept;
  dct:source inspire-lex:PartB05-2;
  rdfs:label "Date of publication"@en;
  rdfs:label "Datum van bekendmaking"@nl;
  skos:definition "This is the date of publication of the resource when available, or the date of entry into force. There may be more than one date of publication."@en;
.
inspire-concept:DateOfLastRevision a skos:Concept;
  dct:source inspire-lex:PartB05-3;
  rdfs:label "Date of last revision"@en;
  rdfs:label "Datum van laatste herziening"@nl;
  skos:definition "This is the date of last revision of the resource, if the resource has been revised. There shall not be more than one date of last revision."@en;
.
inspire-concept:DateOfCreation a skos:Concept;
  dct:source inspire-lex:PartB05-4;
  rdfs:label "Date of creation"@en;
  rdfs:label "Aanmaakdatum"@nl;
  skos:definition "This is the date of creation of the resource. There shall not be more than one date of creation."@en;
.
inspire-concept:Lineage a skos:Concept;
  dct:source inspire-lex:PartB06-1;
  rdfs:label "Lineage"@en;
  rdfs:label "Algemene beschrijving herkomst"@nl;
  skos:definition "This is a statement on process history and/or overall quality of the spatial data set. Where appropriate it may include a statement whether the data set has been validated or quality assured, whether it is the official version (if multiple versions exist), and whether it has legal validity."@en;
  skos:scopeNote "The value domain of this metadata element is free text."@en;
.
inspire-concept:SpatialResolution a skos:Concept;
  dct:source inspire-lex:PartB06-2;
  rdfs:label "Spatial resolution"@en;
  rdfs:label "Ruimtelijke resolutie"@nl;
  skos:definition "Spatial resolution refers to the level of detail of the data set. It shall be expressed as a set of zero to many resolution distances (typically for gridded data and imagery-derived products) or equivalent scales (typically for maps or map-derived products)."@en;
  skos:scopeNote "An equivalent scale is generally expressed as an integer value expressing the scale denominator. A resolution distance shall be expressed as a numerical value associated with a unit of length."@en;
.
inspire-concept:Conformity a skos:Concept;
  dct:source inspire-lex:PartB07;
  rdfs:label "Conformity"@en;
  rdfs:label "Overeenstemming"@nl;
  skos:definition "The requirements referred to in Article 5(2)(a) and Article 11(2)(d) of Directive 2007/2/EC relating to the conformity, and the degree of conformity, with implementing rules adopted under Article 7(1) of Directive 2007/2/EC shall be addressed by the following metadata elements [in sections 7.1 and 7.2]"@en;
.
inspire-concept:ConformitySpecification a skos:Concept;
  dct:source inspire-lex:PartB07-1;
  rdfs:label "Comformity specification"@en;
  rdfs:label "Specificatie van de overeenstemming"@nl;
  skos:definition "This is a citation of the implementing rules adopted under Article 7(1) of Directive 2007/2/EC or other specification to which a particular resource conforms."@en;
  skos:scopeNote "A resource may conform to more than one implementing rules adopted under Article 7(1) of Directive 2007/2/EC or other specification."@en;
  skos:scopeNote "This citation shall include at least the title and a reference date (date of publication, date of last revision or of creation) of the implementing rules adopted under Article 7(1) of Directive 2007/2/EC or of the specification."@en;
.
inspire-concept:ConformityDegree a skos:Concept;
  dct:source inspire-lex:PartB07-2;
  rdfs:label "Conformity degree"@en;
  rdfs:label "Conformiteitsindicatie met de specificatie"@nl;
  skos:definition "This is the degree of conformity of the resource to the implementing rules adopted under Article 7(1) of Directive 2007/2/EC or other specification."@en;
  skos:scopeNote "The value domain of this metadata element is defined in Part D.5"@en;
.
inspire-concept:ConditionsApplyingToAccessAndUse a skos:Concept;
  dct:source inspire-lex:PartB08-1;
  rdfs:label "Conditions applying to access and use"@en;
  rdfs:label "Voorwaarden voor toegang en gebruik"@nl;
  skos:definition "This metadata element defines the conditions for access and use of spatial data sets and services, and where applicable, corresponding fees as required by Article 5(2)(b) and Article 11(2)(f) of Directive 2007/2/EC."@en;
  skos:scopeNote "The value domain of this metadata element is free text. The element must have values. If no conditions apply to the access and use of the resource, 'no conditions apply' shall be used. If conditions are unknown, 'conditions unknown' shall be used. This element shall also provide information on any fees necessary to access and use the resource, if applicable, or refer to a uniform resource locator (URL) where information on fees is available."@en;
.
inspire-collection:AccessAndUseConditions a skos:Collection;
  dct:source inspire-lex:PartB08-1;
  rdfs:label "Access and use conditions"@en;
  skos:member inspire-concept:ConditionsUnknown;
  skos:member inspire-concept:NoConditions;
  skos:member inspire-concept:OtherRestrictions;
.
inspire-concept:ConditionsUnknown a skos:Concept;
  rdfs:label "Conditions unknown"@en;
.
inspire-concept:NoConditions a skos:Concept;
  rdfs:label "No conditions"@en;
.
# The value other restrictions is used in case a "real" condition is stated as free text (see section 2.3.7 of the TG)
inspire-concept:OtherRestrictions a skos:Concept;
  rdfs:label "Other restrictions"@en;
.
  
inspire-concept:LimitationsOnPublicAccess a skos:Concept;
  dct:source inspire-lex:PartB08-2;
  rdfs:label "Limitations on public access"@en;
  rdfs:label "Beperkingen op openbare toegang"@nl;
  skos:definition "When Member States limit public access to spatial data sets and spatial data services under Article 13 of Directive 2007/2/EC, this metadata element shall provide information on the limitations and the reasons for them."@en;
  skos:scopeNote "If there are no limitations on public access, this metadata element shall indicate that fact. The value domain of this metadata element is free text."@en;
.
inspire-concept:ResponsibleOrganisation a skos:Concept;
  dct:source inspire-lex:PartB09;
  rdfs:label "Responsible organisation"@en;
  rdfs:label "Verantwoordelijke organisatie"@nl;
  skos:definition "For the purposes of Article 5(2)(d) and Article 11(2)(g) of Directive 2007/2/EC, the following two metadata elements shall be provided: [in sections 9.1 and 9.2]"@en;
.
  
inspire-concept:ResponsibleParty a skos:Concept;
  dct:source inspire-lex:PartB09-1;
  rdfs:label "Responsible party"@en;
  rdfs:label "Verantwoordelijke organisatie bron"@nl;
  skos:definition "This is the description of the organisation responsible for the establishment, management, maintenance and distribution of the resource."@en;
  skos:scopeNote "This description shall include: (a) the name of the organisation as free text, (b) a contact e-mail address as a character string."@en;
.
inspire-concept:ResponsiblePartyRole a skos:Concept;
  dct:source inspire-lex:PartB09-2;
  rdfs:label "Responsible party role"@en;
  rdfs:label "Rol van de verantwoordelijke organisatie bron"@nl;
  skos:definition "This is the role of the responsible organisation."@en;
  skos:scopeNote "The value domain of this metadata element is defined in Part D.6"@en;
.
inspire-concept:MetadataPointOfContact a skos:Concept;
  dct:source inspire-lex:PartB10-1;
  rdfs:label "Metadata point of contact"@en;
  rdfs:label "Contactpunt voor metagegevens"@nl;
  skos:definition "This is the description of the organisation responsible for the creation and maintenance of the metadata."@en;
  skos:scopeNote "This description shall include: (a) the name of the organisation as free text, (b) a contact e-mail address as a character string."@en;
.
inspire-concept:MetadataDate a skos:Concept;
  dct:source inspire-lex:PartB10-2;
  rdfs:label "Metadata date"@en;
  rdfs:label "Datum van metagegevens"@nl;
  skos:definition "The date which specifies when the metadata record was created or updated."@en;
  skos:scopeNote "This date shall be expressed in conformity with ISO 8601."@en;
.
inspire-concept:MetadataLanguage a skos:Concept;
  dct:source inspire-lex:PartB10-3;
  rdfs:label "Metadata language"@en;
  rdfs:label "Taal van metagegevens"@nl;
  skos:definition "This is the language in which the metadata elements are expressed."@en;
  skos:scopeNote "The value domain of this metadata element is limited to the official languages of the Community expressed in conformity with ISO 639-2."@en;
.

#
# Part D
#

#
# Part D.1
#
inspire-collection:ResourceTypes a skos:Collection;
  dct:source inspire-lex:PartD1;
  rdfs:label "Resource types"@en;
  skos:member inspire-concept:SpatialDatasetSeries;
  skos:member inspire-concept:SpatialDataset;
  skos:member inspire-concept:SpatialService;
.
inspire-concept:SpatialDatasetSeries a skos:Concept;
  dct:source inspire-lex:PartD1-1;
  dct:source inspire-lex:PartA1;
  rdfs:label "Spatial dataset series"@en;
  rdfs:label "Reeks verzamelingen ruimtelijke gegevens"@nl;
  skos:notation "series";
  skos:definition "A collection of spatial data sets sharing the same product specification."@en; #Definition is from inspire-lex:PartA1;
.
inspire-concept:SpatialDataset a skos:Concept;
  dct:source inspire-lex:PartD1-2;
  rdfs:label "Spatial data set"@en;
  rdfs:label "Verzameling ruimtelijke gegevens"@nl;
  skos:notation "dataset";
.
inspire-concept:SpatialService a skos:Concept;
  dct:source inspire-lex:PartD1-3;
  rdfs:label "Spatial service"@en;
  rdfs:label "Dienst met betrekking tot ruimtelijke gegevens"@nl;
  skos:notation "service";
.

#
# Part D.2
#
inspire-collection:TopicCategories a skos:Collection;
  dct:source inspire-lex:PartD2;
  rdfs:label "Topic categories"@en;
  skos:member inspire-concept:Farming;
  skos:member inspire-concept:Biota;
  skos:member inspire-concept:Boundaries;
  skos:member inspire-concept:ClimatologyMeteorologyAtmosphere;
  skos:member inspire-concept:Economy;
  skos:member inspire-concept:Elevation;
  skos:member inspire-concept:Environment;
  skos:member inspire-concept:GeoscientificInformation;
  skos:member inspire-concept:Health;
  skos:member inspire-concept:ImageryBaseMapsEarthCover;
  skos:member inspire-concept:IntelligenceMilitary;
  skos:member inspire-concept:InlandWaters;
  skos:member inspire-concept:Location;
  skos:member inspire-concept:Oceans;
  skos:member inspire-concept:PlanningCadastre;
  skos:member inspire-concept:Society;
  skos:member inspire-concept:Structure;
  skos:member inspire-concept:Transportation;
  skos:member inspire-concept:Utilities;
.
inspire-concept:Farming a skos:Concept;
  dct-source inspire-lex:PartD2-1;
  rdfs:label "Farming"@en;
  rdfs:label "Landbouw en veeteelt"@nl;
  skos:notation "farming";
.
# TODO: Overige TopicCategories opnemen

#
# Part D.3
#
inspire-collection:SpatialDataServiceTypes a skos:Collection;
  dct:source inspire-lex:PartD3;
  rdfs:label "Spatial data service types"@en;
  skos:member inspire-concept:DiscoveryService;
  skos:member inspire-concept:ViewService;
  skos:member inspire-concept:DownloadService;
  skos:member inspire-concept:TransformationService;
  skos:member inspire-concept:InvokeSpatialDataService;
  skos:member inspire-concept:OtherService;
.
inspire-concept:DiscoveryService a skos:Concept;
  dct-source inspire-lex:PartD3-1;
  rdfs:label "Discovery service"@en;
  rdfs:label "Zoekdienst"@nl;
  skos:definition "Services making it possible to search for spatial data sets and services on the basis of the content of the corresponding metadata and to display the content of the metadata."@en;
  skos:notation "discovery";
.
inspire-concept:ViewService a skos:Concept;
  dct-source inspire-lex:PartD3-2;
  rdfs:label "View service"@en;
  rdfs:label "Raadpleegdienst"@nl;
  skos:definition "Service that makes it possible, as a minimum, to display, navigate, zoom in and out, pan or overlay viewable spatial data sets and to display legend information and any relevant content of metadata."@en;
  skos:notation "view";
.
inspire-concept:DownloadService a skos:Concept;
  dct-source inspire-lex:PartD3-3;
  rdfs:label "Download service"@en;
  rdfs:label "Downloaddienst"@nl;
  skos:definition "Service that enables copies of spatial data sets, or parts of such sets, to be downloaded and, where practicable, accessed directly."@en;
  skos:notation "download";
.
inspire-concept:TransformationService a skos:Concept;
  dct-source inspire-lex:PartD3-4;
  rdfs:label "Transformation service"@en;
  rdfs:label "Verwerkingsdienst"@nl;
  skos:definition "Service that enables spatial data sets to be transformed with a view to achieving interoperability."@en;
  skos:notation "transformation";
.
inspire-concept:InvokeSpatialDataService a skos:Concept;
  dct-source inspire-lex:PartD3-5;
  rdfs:label "Invoke spatial data service"@en;
  rdfs:label "Oproepdienst"@nl;
  skos:definition "Service that allows defining both the data inputs and data outputs expected by the spatial service and a workflow or service chain combining multiple services. It also allows defining the external web service interface of the workflow or service chain."@en;
  skos:notation "invoke";
.
inspire-concept:OtherService a skos:Concept;
  dct-source inspire-lex:PartD3-6;
  rdfs:label "Other service"@en;
  rdfs:label "Andere dienst"@nl;
  skos:definition ""@en;
  skos:notation "other";
.

#
# Part D.4
#
inspire-collection:ClassificationOfSpatialDataServices a skos:Collection;
  rdfs:label "Classification of spatial data services"@en;
  skos:definition "The keywords are based on the geographic services taxonomy of EN ISO 19119. This taxonomy is organised in categories, the subcategories defining the value domain of the classification of spatial data services."@en;
  skos:member inspire-concept:GeographicHumanInteractionServices;
  skos:member inspire-concept:CatalogueViewer;
  skos:member inspire-concept:GeographicViewer;
  skos:member inspire-concept:GeographicSpreadsheetViewer;
  skos:member inspire-concept:ServiceEditor;
  #TODO Compleet maken
.
inspire-concept:GeographicHumanInteractionServices a skos:Concept;
  rdfs:label "Geographic human interaction services"@en;
  skos:notation "humanInteractionService";
.
inspire-concept:CatalogueViewer a skos:Concept;
  rdfs:label "Catalogue viewer"@en;
  skos:definition "Client service that allows a user to interact with a catalogue to locate, browse, and manage metadata about geographic data or geographic services."@en;
  skos:notation "humanCatalogueViewer";
  skos:broader inspire-concept:GeographicHumanInteractionServices;
.

#
# Part D.5
#
inspire-collection:DegreeOfComformity a skos:Collection;
  rdfs:label "Degree of comformity"@en;
  skos:member inspire-concept:Conformant;
  skos:member inspire-concept:NotConformant;
  skos:member inspire-concept:NotEvaluated;
.
inspire-concept:Conformant a skos:Concept;
  rdfs:label "Conformant"@en;
  skos:definition "The resource is fully conformant with the cited specification."@en;
  skos:notation "conformant";
.
inspire-concept:NotConformant a skos:Concept;
  rdfs:label "Not conformant"@en;
  skos:definition "The resource does not conform to the cited specification."@en;
  skos:notation "notConformant";
.
inspire-concept:NotEvaluated a skos:Concept;
  rdfs:label "Not evaluated"@en;
  skos:definition "Conformance has not been evaluated."@en;
  skos:notation "notEvaluated";
.

#
# Part D.6
#
inspire-collection:ResponsiblePartyRoles a skos:Collection;
  rdfs:label "Responsible party roles"@en;
  skos:member inspire-concept:ResourceProvider;
  skos:member inspire-concept:Custodian;
  skos:member inspire-concept:Owner;
  skos:member inspire-concept:User;
  skos:member inspire-concept:Distributor;
  skos:member inspire-concept:Originator;
  skos:member inspire-concept:PointOfContact;
  skos:member inspire-concept:PrincipalInvestigator;
  skos:member inspire-concept:Processor;
  skos:member inspire-concept:Publisher;
  skos:member inspire-concept:Author;
.
#TODO Compleet maken
inspire-concept:ResourceProvider a skos:Concept;
  rdfs:label "Resource provider"@en;
  skos:definition "Party that supplies the resource."@en;
  skos:notation "resourceProvider";
.
inspire-concept:Custodian a skos:Concept;
  rdfs:label "Custodian"@en;
  skos:definition "Party that accepts accountability and responsibility for the data and ensures appropriate care and maintenance of the resource."@en;
  skos:notation "custodian";
.
inspire-concept:Owner a skos:Concept;
  rdfs:label "Owner"@en;
  skos:definition "Party that owns the resource."@en;
  skos:notation "owner";
.
inspire-concept:User a skos:Concept;
  rdfs:label "User"@en;
  skos:definition "Party who uses the resource."@en;
  skos:notation "user";
.
inspire-concept:Distributor a skos:Concept;
  rdfs:label "Distributor"@en;
  skos:definition "Party who distributes the resource."@en;
  skos:notation "distributor";
.
inspire-concept:Originator a skos:Concept;
  rdfs:label "Originator"@en;
  skos:definition "Party who created the resource"@en;
  skos:notation "originator";
.
inspire-concept:PointOfContact a skos:Concept;
  rdfs:label "Point of Contact"@en;
  skos:definition "Party who can be contacted for acquiring knowledge about or acquisition of the resource."@en;
  skos:notation "pointOfContact";
.
inspire-concept:PrincipalInvestigator a skos:Concept;
  rdfs:label "Principal Investigator"@en;
  skos:definition "Key party responsible for gathering information and conducting research."@en;
  skos:notation "principalInvestigator";
.
inspire-concept:Processor a skos:Concept;
  rdfs:label "Processor"@en;
  skos:definition "Party who has processed the data in a manner such that the resource has been modified."@en;
  skos:notation "processor";
.
inspire-concept:Publisher a skos:Concept;
  rdfs:label "Publisher"@en;
  skos:definition "Party who published the resource."@en;
  skos:notation "publisher";
.
inspire-concept:Author a skos:Concept;
  rdfs:label "Author"@en;
  skos:definition "Party who authored the resource."@en;
  skos:notation "author";
.
inspire-concept: a skos:Concept;
  rdfs:label ""@en;
  skos:definition ""@en;
  skos:notation "";
.
inspire-concept: a skos:Concept;
  rdfs:label ""@en;
  skos:definition ""@en;
  skos:notation "";
.
inspire-concept: a skos:Concept;
  rdfs:label ""@en;
  skos:definition ""@en;
  skos:notation "";
.
inspire-concept: a skos:Concept;
  rdfs:label ""@en;
  skos:definition ""@en;
  skos:notation "";
.
inspire-concept: a skos:Concept;
  rdfs:label ""@en;
  skos:definition ""@en;
  skos:notation "";
.

#
# Artikel 2 definities
#
inspire-concept:CodeList a skos:Concept;
  dct:source inspire-lex:Article02-05;
  rdfs:label "Code list"@en;
  rdfs:label "Codelijst"@nl;
  skos:definition "an open enumeration that can be extended";
.
inspire-concept:Enumeration a skos:Concept;
  dct:source inspire-lex:Article02-07;
  rdfs:label "Enumeration"@en;
  rdfs:label "Opsomming"@nl;
  skos:definition "a data type whose instances form a fixed list of named literal values. Attributes of an enumerated type may only take values from this list";
.
inspire-concept:EndPoint a skos:Concept;
  dct:source inspire-lex:Article02-31;
  rdfs:label "End point"@en;
  rdfs:label "Eindpunt"@nl;
  skos:definition "the internet address used to directly call an operation provided by a spatial data service";
.
inspire-concept:AccessPoint a skos:Concept;
  dct:source inspire-lex:Article02-32;
  rdfs:label "Access point"@en;
  rdfs:label "Toegangspunt"@nl;
  skos:definition "an internet address containing a detailed description of a spatial data service, including a list of end points to allow its execution";
.
#
# Artikel 13
#
inspire-concept:SpatialDatasetCoordinateReferenceSystem a skos:Concept;
  dct:source inspire-lex:Article13-1;
  rdfs:label "Spatial data set Coordinate Reference System"@en;
  rdfs:label "Coördinaatreferentiesysteem van de verzameling ruimtelijke gegevens"@nl;
  skos:definition "Description of the coordinate reference system(s) used in the data set."@en;
  skos:definition "Beschrijving van het (de) in de gegevensverzameling gebruikte coördinaatreferentiesyste(e)m(en)."@nl;
.
inspire-concept:SpatialDatasetTemporalReferenceSystem a skos:Concept;
  dct:source inspire-lex:Article13-2;
  rdfs:label "Spatial data set Temporal Reference System"@en;
  rdfs:label "Tijdsreferentiesysteem van de verzameling ruimtelijke gegevens"@nl;
  skos:definition "Description of the temporal reference system(s) used in the data set."@en;
  skos:scopeNote "This element is mandatory only if the spatial data set contains temporal information that does not refer to the default temporal reference system."@en;
.
inspire-concept:SpatialDatasetEncoding a skos:Concept;
  dct:source inspire-lex:Article13-3;
  rdfs:label "Spatial data set encoding"@en;
  rdfs:label "Codering van de verzameling ruimtelijke gegevens"@nl;
  skos:definition "Description of the computer language construct(s) specifying the representation of data objects in a record, file, message, storage device or transmission channel."@en;
.
inspire-concept:SpatialDatasetTopologicalConsistency a skos:Concept;
  dct:source inspire-lex:Article13-4;
  rdfs:label "Spatial data set topological consistency"@en;
  rdfs:label "Topologische consistentie van de verzameling ruimtelijke gegevens"@nl;
  skos:definition "Correctness of the explicitly encoded topological characteristics of the data set as described by the scope."@en;
  skos:scopeNote "This element is mandatory only if the data set includes types from the Generic Network Model and does not assure centreline topology (connectivity of centrelines) for the network."@en;
.
inspire-concept:SpatialDatasetCharacterEncoding a skos:Concept;
  dct:source inspire-lex:Article13-5;
  rdfs:label "Spatial data set character encoding"@en;
  rdfs:label "Tekencodering van de verzameling ruimtelijke gegevens"@nl;
  skos:definition "The character encoding used in the data set."@en;
  skos:scopeNote "This element is mandatory only if an encoding is used that is not based on UTF-8."@en;
.
inspire-concept:SpatialDatasetSpatialRepresentationType a skos:Concept;
  dct:source inspire-lex:Article13-6;
  rdfs:label "Spatial data set representation type"@en;
  rdfs:label "Ruimtelijk weergavetype van de verzameling ruimtelijke gegevens"@nl;
  skos:definition "The method used to spatially represent geographic information."@en;
.

#
# Artikel 14a, verwijzing naar Annex V Part B
#
inspire-concept:SpatialDataServicesCategory a skos:Concept;
  dct:source inspire-lex:AnnexVPartB1;
  rdfs:label "Spatial data services category"@en;
  skos:definition "This is a citation of the status of the spatial data service versus invocability."@en;
  skos:scopeNote "The value domain of this metadata element is as follows: (a) invocabule; (b) interoperable; (c) harmonised"@en;
.
inspire-collection:SpatialDataServicesCategories a skos:Collection;
  rdfs:label "Spatial data services categories"@en;
  dct:source inspire-lex:AnnexVPartB1;
  skos:member inspire-concept:Invocable;
  skos:member inspire-concept:Interoperable;
  skos:member inspire-concept:Harmonised
.
inspire-concept:Invocable a skos:Concept;
  dct:source inspire-lex:AnnexVPartB1-1;
  rdfs:label "Invocable"@en;
  rdfs:label "Aanroepbaar"@nl;
  skos:definition "The spatial data service is an invocable spatial data service."@en;
  skos:notation "invocable";
.
inspire-concept:Interoperable a skos:Concept;
  dct:source inspire-lex:AnnexVPartB1-2;
  rdfs:label "Interoperable"@en;
  rdfs:label "Interoperabel"@nl;
  skos:definition "The invocable spatial data service is an interoperable spatial data service."@en;
  skos:notation "interoperable";
  skos:broader inspire-concept:Invocable;
.
inspire-concept:Harmonised a skos:Concept;
  dct:source inspire-lex:AnnexVPartB1-3;
  rdfs:label "Harmonised"@en;
  rdfs:label "Geharmoniseerd"@nl;
  skos:definition "The interoperable spatial data service is a harmonised spatial data service."@en;
  skos:notation "harmonised";
  skos:broader inspire-concept:Interoperable;
.

#
# Artikel 14b, voor wat betreft de verwijzing naar Annex VI Part B
#
inspire-concept:CoordinateReferenceSystemIdentifier a skos:Concept;
  dct:source inspire-lex:AnnexVIPartB3;
  rdfs:label "Coordinate Reference System Identifier"@en;
  skos:definition "Where appropriate, this is the list of coordinate reference systems supported by the spatial data service."@en;
  skos:scopeNote "Each supported coordinate reference system shall be expressed using an identifier."@en;
.
inspire-concept:QualityOfService a skos:Concept;
  dct:source inspire-lex:AnnexVIPartB4;
  rdfs:label "Quality of Service"@en;
  skos:definition "This is the minimum quality of service estimated by the spatial data service responsible party and expected to be valid over a period of time."@en;
.
inspire-concept:QualityOfServiceCriteria a skos:Concept;
  dct:source inspire-lex:AnnexVIPartB4-1;
  rdfs:label "Quality of Service Criteria"@en;
  skos:definition "These are the criteria to which the measurements refer."@en;
  skos:scopeNote "The value domain of this metadata element is as follows: [availability, performance, capacity]"@en;
.
inspire-collection:QualityOfServiceCriteriaCodes a skos:Collection;
  dct:source inspire-lex:AnnexVIPartB4-1;
  rdfs:label "Quality of Service Criteria Codes"@en;
  skos:member inspire-concept:Availability;
  skos:member inspire-concept:Performance;
  skos:member inspire-concept:Capacity;
.
inspire-concept:Availability a skos:Concept;
  dct:source inspire-lex:AnnexVIPartB4-1-1;
  rdfs:label "Availability"@en;
  skos:definition "It describes the percentage of time the service is available."@en;
.
inspire-concept:Performance a skos:Concept;
  dct:source inspire-lex:AnnexVIPartB4-1-2;
  rdfs:label "Performance"@en;
  skos:definition "It describes how fast a request to the spatial data service can be completed."@en;
.
inspire-concept:Capacity a skos:Concept;
  dct:source inspire-lex:AnnexVIPartB4-1-3;
  rdfs:label "Capacity"@en;
  skos:definition "It describes the maximum number of simultaneous requests that can be completed with the declared performance."@en;
.
inspire-concept:QualityOfServiceMeasurementDescription a skos:Concept;
  dct:source inspire-lex:AnnexVIPartB4-2-1;
  rdfs:label "Quality of Service Measurement Description"@en;
  skos:definition "It describes the measurement for each criterion."@en;
  skos:scopeNote "The value domain of this metadata element is free text."@en;
.
inspire-concept:QualityOfServiceMeasurementValue a skos:Concept;
  dct:source inspire-lex:AnnexVIPartB4-2-2;
  rdfs:label "Quality of Service Measurement Value"@en;
  skos:definition "It describes the value of the measurement for each criterion."@en;
  skos:scopeNote "The value domain of this metadata element is free text."@en;
  skos:notation "value";
.
inspire-concept:QualityOfServiceMeasurementUnit a skos:Concept;
  dct:source inspire-lex:AnnexVIPartB4-2-3;
  rdfs:label "Quality of Service Measurement Unit"@en;
  skos:definition "It describes the Unit of the measurement for each criterion."@en;
  skos:scopeNote "The value domain of this metadata element is free text."@en;
  skos:notation "unit";
.

#
# Artikel 14b, voor wat betreft de verwijzing naar Annex VII Part B
#
inspire-concept:InvocationMetadata a skos:Concept;
  dct:source inspire-lex:AnnexVIIPartB3;
  rdfs:label "Invocation metadata"@en;
  skos:definition "The invocation metadata element documents the interfaces of the harmonised spatial data service and lists the end points to enable machine-to machine communication."@en;
.

# =================================
# Shapes vanuit implementatie
# =================================

inspire:Resource a owl:Class;
  rdfs:label "Resource";
.
inspire:Dataset a owl:Class;
  rdfs:label "Dataset";
  rdfs:subClassOf inspire:Resource;
.
inspire:Service a owl:Class;
  rdfs:label "Service";
  rdfs:subClassOf inspire:Resource;
.

#
# Section C.2 of Technical Guidance for the implementation of INSPIRE dataset and service metadata based on ISO/TS 19139:2007
#

inspire-shape:Resource a sh:NodeShape;
  dct:subject inspire-concept:Resource;
  sh:name "+Resource";
  sh:targetClass inspire:Resource;
  inspire-meta:xpath "/";
  sh:property inspire-shape:ResourceTitle;
  sh:property inspire-shape:ResourceAbstract;
  sh:property inspire-shape:ResourceType;
  sh:property inspire-shape:Keyword;
  sh:property inspire-shape:GeographicBoundingBox;
  sh:property inspire-shape:TemporalExtent;
  sh:property inspire-shape:DateOfPublication;
  sh:property inspire-shape:DateOfLastRevision;
  sh:property inspire-shape:DateOfCreation;
  sh:property inspire-shape:SpatialResolutionEquivalentScale;
  sh:property inspire-shape:SpatialResolutionDistance;
  sh:property inspire-shape:Conformity;
  sh:property inspire-shape:ConditionsApplyingToAccessAndUse;
  sh:property inspire-shape:ConditionsApplyingToAccessAndUseOtherConstraints;
  sh:property inspire-shape:ConditionsApplyingToUse;
  sh:property inspire-shape:ConditionsApplyingToUseOtherConstraints;
  sh:property inspire-shape:LimitationsOnPublicAccess;
  sh:property inspire-shape:LimitationsOnPublicAccessOtherConstraints;
  sh:property inspire-shape:ResponsibleOrganisation;
  sh:property inspire-shape:MetadataPointOfContact;
  sh:property inspire-shape:MetadataDate;
  sh:property inspire-shape:MetadataLanguage;
.
inspire-shape:Dataset a sh:NodeShape;
  dct:subject inspire-concept:Dataset;
  sh:name "+Dataset(series)";
  sh:targetClass inspire:Dataset;
  inspire-meta:xpath "/";
  sh:property inspire-shape:ResourceLocator; # Lijkt erop dat dit niet voor services geldt?
  sh:property inspire-shape:ResourceLocatorComplex;
  sh:property inspire-shape:UniqueResourceIdentifier;
  sh:property inspire-shape:ResourceLanguage;
  sh:property inspire-shape:TopicCategory;
  sh:property inspire-shape:Lineage;
  sh:property inspire-shape:SpatialDatasetCoordinateReferenceSystem;
  sh:property inspire-shape:SpatialDatasetTemporalReferenceSystem;
  sh:property inspire-shape:SpatialDatasetEncoding;
  sh:property inspire-shape:SpatialDatasetCharacterEncoding;
  sh:property inspire-shape:SpatialDatasetSpatialRepresentationType;
  sh:property inspire-shape:SpatialDatasetTopologicalConsistencyQuantitive;
  sh:property inspire-shape:SpatialDatasetTopologicalConsistencyDescriptive;
.
inspire-shape:Service a sh:NodeShape;
  dct:subject inspire-concept:Service;
  sh:name "+Service";
  sh:targetClass inspire:Service;
  inspire-meta:xpath "/";
  sh:property inspire-shape:CoupledResource;
  sh:property inspire-shape:SpatialDataServiceType;
  sh:property inspire-shape:SpatialDataServicesCategory;
  sh:property inspire-shape:CoordinateReferenceSystemIdentifier;
  sh:property inspire-shape:QualityOfService;
  sh:property inspire-shape:OperationName;
  sh:property inspire-shape:DCP;
  sh:property inspire-shape:ConnectPoint;
.
inspire-shape:ResourceTitle a sh:PropertyShape;
  dct:subject inspire-concept:ResourceTitle;
  sh:name "title";
  sh:severity sh:Violation;
  sh:datatype xsd:string; #CharacterString
  sh:node inspire-shape:FreeText;
  sh:minCount 1;
  sh:maxCount 1;
  inspire-meta:isoref "360. title";
  inspire-meta:xpath "identificationInfo[1]/*/citation/*/title";
  skos:example "SPI: Standardized Precipitation Index";
.
inspire-shape:ResourceAbstract a sh:PropertyShape;
  dct:subject inspire-concept:ResourceAbstract;
  sh:name "abstract";
  sh:severity sh:Violation;
  sh:datatype xsd:string; #CharacterString
  sh:node inspire-shape:FreeText;
  sh:minCount 1;
  sh:maxCount 1;
  inspire-meta:isoref "25. abstract";
  inspire-meta:xpath "identificationInfo[1]/*/abstract";
  skos:example "The Standardized Precipitation Index (SPI-n) is a statistical indicator comparing the total precipitation received at a particular location during a period of n months with the long-term rainfall distribution for the same period of time at that location. SPI is calculated on a monthly basis for a moving window of n months, where n indicates the rainfall accumulation period, which is typically 1, 3, 6, 9, 12, 24 or 48 months. The corresponding SPIs are denoted as SPI-1, SPI-3, SPI-6, etc. In order to allow for the statistical comparison of wetter and drier climates, SPI is based on a transformation of the accumulated precipitation into a standard normal variable with zero mean and variance equal to one. SPI results are given in units of standard deviation from the long-term mean of the standardized distribution. In 2010 WMO selected the SPI as a key meteorological drought indicator to be produced operationally by meteorological services";
.
inspire-shape:ResourceType a sh:PropertyShape;
  dct:subject inspire-concept:ResourceType;
  sh:name "type";
  sh:severity sh:Violation;
  sh:class skos:Concept; #MD_ScopeCode
  sh:node inspire-shape:ResourceTypes;
  sh:minCount 1;
  sh:maxCount 1;
  inspire-meta:isoref "6. hierarchyLevel";
  inspire-meta:xpath "hierarchyLevel";
  skos:example "dataset";
.
inspire-shape:ResourceLocator a sh:PropertyShape;
  dct:subject inspire-concept:ResourceLocator;
  sh:name "locator";
  sh:severity sh:Warning;
  sh:datatype xsd:anyURI; #URL
  sh:node inspire-shape:URL;
  inspire-meta:isoref "397. linkage";
  inspire-meta:xpath "distributionInfo/*/transferOptions/*/onLine/*/linkage";
  skos:example "http://edo.jrc.ec.europa.eu/chm/ows.php?VERSION=1.3.0&SERVICE=WMS&REQUEST=GetCapabilities";
  skos:example "http://www.eea.europa.eu/data-and-maps/data/wise-river-basin-districts-rbds-1";
  rdfs:comment '''A Resource Locator could be described, moreover, by other additional elements as a Title, a Description and a Function. In that case, the Title and the Description shall be free text and the Function shall be filled by the CI_OnLineFunctionCode (ISO 19115 code list).
Examples of Resource Locator with these additional elements:
- JRC EDO (European Drought Observatory) - Drought Indexes WMS
  - Linkage: http://edo.jrc.ec.europa.eu/chm/ows.php?VERSION=1.3.0&SERVICE=WMS&REQUEST=GetCapabilities
- Title: JRC EDO (European Drought Observatory) - Drought Indexes WMS
- Description: WMS delivering maps of drought indexes provided by the European Drought Observatory (EDO).
- Function: information
- WISE River basin districts (RBDs)
  - Linkage: http://www.eea.europa.eu/data-and-maps/data/wise-river-basin-districts-rbds-1
  - Title: WISE River basin districts (RBDs)
  - Description: Version 1.4 (06/2011) - River Basin Districts (RBDs) and/or their subunits (RBDSUs) are the main units for the management of river basins and have been delineated by Member States under Article 3 and updated by reporting to Article 13 of the Water Framework Directive.
  - Function: information''';
.
inspire-shape:ResourceLocatorComplex a sh:PropertyShape;
  dct:subject inspire-concept:ResourceLocator;
  sh:name "locator";
  sh:node inspire-shape:ResourceLocatorElement;
  sh:nodeKind sh:BlankNode;
  inspire-meta:xpath "distributionInfo/*/transferOptions/*/onLine/*/linkage/";
.
  
inspire-shape:UniqueResourceIdentifier a sh:PropertyShape;
  dct:subject inspire-concept:UniqueResourceIdentifier;
  sh:name "identifier";
  sh:severity sh:Violation; #Only for dataset and dataset series
  sh:node inspire-shape:URI;
  sh:datatype xsd:anyURI; #205. MD_Identifier, domain = URI
  sh:minCount 1; #Only for dataset and dataset series
  inspire-meta:isoref "365. identifier";
  inspire-meta:xpath "identificationInfo[1]/*/citation/*/identifier";
  skos:example "The Unique resource identifier semantically consisting of namespace: https://example.org/ and identifier: ab749859 and is provided together in element code: https://example.org/ab749859";
  rdfs:comment "The unique resource identifier is needed to provide a queryable information when following data-service-coupling (see also 4.1.2.4). Therefore it is necessary to have the identifier itself together with the namespace in element code. The use of RS_Identifier (with a separate element codeSpace) is not suitable here";
.
inspire-shape:CoupledResource a sh:PropertyShape;
  dct:subject inspire-concept:CoupledResource;
  sh:name "coupledResource";
  sh:severity sh:Warning; #Not applicable for datasets and dataset series, mandatory if linkage to datasets on which the service operates are available
  sh:node inspire-shape:Dataset; # 36. MD_DataIdentification, unique resource identifier or locator (URL) of the MD_DataIdentification object
  sh:class inspire:Dataset;
  inspire-meta:isoref "9 of table C.1. operatesOn";
  inspire-meta:xpath "identificationInfo[1]/*/operatesOn";
  skos:example "http://vap-xgeodev.jrc.ec.europa.eu/geonetwork/srv/eng/csw?SERVICE=CSW&VERSION=2.0.2&REQUEST=GetRecordById&ID=f9ee6623-cf4c-11e1-9105-0017085a97ab&OUTPUTSCHEMA=http://www.isotc211.org/2005/gmd&ELEMENTSETNAME=full#lakes";
  rdfs:comment "The implementation of this element by reference means that the xlink:href element are pointing to a metadatarecord that contains a MD_DataIdentification object. The reference to the MD_DataIdentification object is done using the xpointer reference using the #-sign. The example above points to #lakes which is the ID of this object. Check example on xml encoding in section 0. The Unique Resource Identifier for the can be explicilty defined for the target dataset using the optional uuidref.attribute.";
.
inspire-shape:ResourceLanguage a sh:PropertyShape;
  dct:subject inspire-concept:ResourceLanguage;
  sh:name "language";
  sh:severity sh:Warning; # Mandatory if the resource includes textual information, not applicable to services
  sh:datatype xsd:string; # LanguageCode (ISO/TS 19139)
  sh:node inspire-shape:LanguageCode;
  inspire-meta:isoref "39. language";
  inspire-meta:xpath "identificationInfo[1]/*/language";
  skos:example "eng";
.
inspire-shape:TopicCategory a sh:PropertyShape;
  dct:subject inspire-concept:TopicCategory;
  sh:name "topicCategory";
  sh:severity sh:Violation; # Only for dataset and dataset series, not applicable to services
  sh:minCount 1;
  sh:class skos:Concept; # MD_TopicCategory
  sh:node inspire-shape:TopicCategories;
  inspire-meta:isoref "41. topicCategory";
  inspire-meta:xpath "identificationInfo[1]/*/topicCategory";
  skos:example "climatologyMeteorologyAtmosphere";
  rdfs:comment "The topic categories defined in Part D 2 of [Regulation 1205/2008] are derived directly from the topic categories defined in MD_TopicCategoryCode (B.5.27 of ISO 19115)";
.
inspire-shape:SpatialDataServiceType a sh:PropertyShape;
  dct:subject inspire-concept:SpatialDataServiceType;
  sh:name "SDS type";
  sh:severity sh:Violation; # Only for services, not applicable to datasets and dataset series
  sh:class skos:Concept; # GenericName
  sh:minCount 1;
  sh:maxCount 1;
  sh:node inspire-shape:SpatialDataServiceTypes;
  inspire-meta:isoref "1 of table C.1. serviceType";
  inspire-meta:xpath "identificationInfo[1]/*/serviceType";
  skos:example "view";
.
inspire-shape:Keyword a sh:PropertyShape;
  dct:subject inspire-concept:Keyword;
  sh:name "keyword";
  sh:node inspire-shape:KeywordElement;
  sh:nodeKind sh:BlankNode;
  sh:minCount 1;
  inspire-meta:xpath "identificationInfo[1]/*/descriptiveKeywords/*/";
.
inspire-shape:KeywordValue a sh:PropertyShape;
  dct:subject inspire-concept:KeywordValue;
  sh:name "keyword value";
  sh:severity sh:Violation;
  sh:datatype xsd:string;
  sh:node inspire-shape:FreeText;
  sh:minCount 1;
  sh:maxCount 1; #Dit is niet geheel duidelijk, kan ook zijn dat er meerdere keywordvalues mogen zijn, mits uit dezelfde vocabulary
  inspire-meta:isoref "53. keyword";
  inspire-meta:xpath "identificationInfo[1]/*/descriptiveKeywords/*/keyword";
  skos:example "Atmospheric conditions (INSPIRE Spatial Data Theme)";
  skos:example "humanCatalogueViewer (spatial data service subcategory)";
  skos:example "water springs (AGROVOC)";
  skos:example "rain water (GEMET Concepts)";
  rdfs:comment "Each instance of ISO 19115 keyword may originate from a controlled vocabulary described through the thesaurusName property of the instance of descriptiveKeywords to which the keyword pertains";
.
inspire-shape:KeywordOriginatingControlledVocabulary a sh:PropertyShape;
  dct:subject inspire-concept:KeywordOriginatingControlledVocabulary;
  sh:name "originating controlled vocabulary";
  sh:severity sh:Warning; # Mandatory if keyword is from controlled vocabulary
  sh:node inspire-shape:Citation;
  sh:nodeKind sh:BlankNode;
  sh:maxCount 1;
  inspire-meta:isoref "55. thesaurusName";
  inspire-meta:xpath "identificationInfo[1]/*/descriptiveKeywords/*/thesaurusName";
  skos:example '''Identification for a keyword originating from GEMET- INSPIRE themes:
- title: GEMET - INSPIRE themes, version 1.0
- date:
  - dateType: publication
  - date: 2008-06-01";
  skos:example "Identification for a keyword originating from GEMET - Concepts:
- title: GEMET - Concepts, version 2.4
- date:
  - dateType: publication
  - date: 2010-01-13";
  skos:example "Identification for a keyword originating from AGROVOC:
- title: AGROVOC
- date:
    - dateType: publication
    - date: 2008-04-14''';
.
inspire-shape:GeographicBoundingBox a sh:PropertyShape;
  dct:subject inspire-concept:GeographicBoundingBox;
  sh:name "geographicBoundingBox";
  sh:severity sh:Violation; # Mandatory for datasets and spatial dataset series, Conditional for spatial services: mandatory for services with an explicit geographic extent
  sh:node inspire-shape:BoundingBox;
  sh:nodeKind sh:BlankNode;
  inspire-meta:isoref "344. westBoundLongitude";
  inspire-meta:isoref "345. eastBoundLongitude";
  inspire-meta:isoref "346. southBoundLatitude";
  inspire-meta:isoref "347. northBoundLatitude";
  inspire-meta:xpath "identificationInfo[1]/*/extent/*/geographicElement/*/westBoundLongitude";
  inspire-meta:xpath "identificationInfo[1]/*/extent/*/geographicElement/*/eastBoundLongitude";
  inspire-meta:xpath "identificationInfo[1]/*/extent/*/geographicElement/*/southBoundLatitude";
  inspire-meta:xpath "identificationInfo[1]/*/extent/*/geographicElement/*/northBoundLatitude";
  skos:example "-15.00 (westBoundLongitude)";
  skos:example "45.00 (eastBoundLongitude)";
  skos:example "35.00 (southBoundLatitude)";
  skos:example "72.00 (northBoundLatitude)";
  rdfs:comment '''- There may be as many bounding boxes defining the geographic location of the resource as instances of identificationInfo[1]/*/extent/*/geographicElement having the westBoundLongitude, eastBoundLongitude, southBoundLatitude and northBoundLatitude properties. The four coordinates of the bounding box originate from the same instance.
- If the bounding box crosses the 180 meridian, then the value of the westBoundLongitude will be greater than the eastBoundLongitude value.'''
.
inspire-shape:TemporalExtent a sh:PropertyShape;
  dct:subject inspire-concept:TemporalExtent;
  sh:name "temporalExtent";
  sh:severity sh:Warning; #Conditional: At least one temporal reference is required
  sh:node inspire-shape:Period; # TM_Primitive, As described in ISO 19108
  sh:nodeKind sh:BlankNode;
  inspire-meta:isoref "351. extent";
  inspire-meta:xpath "identificationInfo[1]/*/extent/*/temporalElement/*/extent";
  skos:example "From 2008-01-01T11:45:30 to 2008-12-31T09:10:00";
  rdfs:comment "The overall time period covered by the content of the resource may be composed of one or many instances";
.
inspire-shape:DateOfPublication a sh:PropertyShape;
  dct:subject inspire-concept:DateOfPublication;
  sh:name "dateOfPublication";
  sh:node inspire-shape:CIDate;
  sh:severity sh:Warning; #Conditional: at least one date of publication / date of creation / date of revision is required
  sh:datatype xsd:dateTime; #Described in ISO 19108 and ISO 8601
  inspire-meta:isoref "362. date";
  inspire-meta:xpath "identificationInfo[1]/*/citation/*/date[./*/dateType/*/text()='publication']/*/date";
  skos:example "2009-03-15";
  skos:example "2009-03-15T11:15:00";
.
inspire-shape:DateOfLastRevision a sh:PropertyShape;
  dct:subject inspire-concept:DateOfLastRevision;
  sh:name "dateOfLastRevision";
  sh:severity sh:Warning; #Conditional: at least one date of publication / date of creation / date of revision is required
  sh:maxCount 1;
  sh:node inspire-shape:CIDate;
  sh:datatype xsd:dateTime; #Described in ISO 19108 and ISO 8601
  inspire-meta:isoref "362. date";
  inspire-meta:xpath "identificationInfo[1]/*/citation/*/date[./*/dateType/*/text()='publication']/*/date";
  skos:example "2009-04-15";
  skos:example "2009-04-15T11:15:00";
  rdfs:comment "There may be more than one revision date provided in an ISO 19115 metadata, but INSPIRE will consider as date of last revision the more recent one";
.
inspire-shape:DateOfCreation a sh:PropertyShape;
  dct:subject inspire-concept:DateOfCreation;
  sh:name "dateOfCreation";
  sh:severity sh:Warning; #Conditional: at least one date of publication / date of creation / date of revision is required
  sh:maxCount 1;
  sh:node inspire-shape:CIDate;
  sh:datatype xsd:dateTime; #Described in ISO 19108 and ISO 8601
  inspire-meta:isoref "362. date";
  inspire-meta:xpath "identificationInfo[1]/*/citation/*/date[./*/dateType/*/text()='publication']/*/date";
  skos:example "2009-02-15";
  skos:example "2009-02-15T11:15:00";
.
inspire-shape:Lineage a sh:PropertyShape;
  dct:subject inspire-concept:Lineage;
  sh:name "lineage";
  sh:severity sh:Violation; #Mandatory for spatial dataset and spatial dataset series. Not applicable to services.
  sh:minCount 1;
  sh:maxCount 1;
  sh:datatype xsd:string; #CharacterString
  sh:node inspire-shape:FreeText;
  inspire-meta:isoref "83. statement";
  inspire-meta:xpath "dataQualityInfo/*/lineage/*/statement";
  skos:example "Computation of the SPI involves fitting a probability density function to a given frequency distribution of precipitation totals for a station or grid point and for an accumulation period. We use the gamma probability density function. The statistics for the frequency distribution are calculated on the basis of a reference period of at least 30 years. The parameters of the probability density function are then used to find the cumulative probability of the observed precipitation for the required month and temporal scale. This cumulative probability is then transformed to the standardised normal distribution with mean zero and variance one, which results in the value of the SPI. The SPI values are computed using the so-called MARS weather stations as rainfall input data. Refer the MARS weather catalogue for characteristics of the quality and quantity of these data. We only rely on the rainfall data input";
.
inspire-shape:SpatialResolutionEquivalentScale a sh:PropertyShape;
  dct:subject inspire-concept:SpatialResolution;
  sh:name "spatialResolution";
  sh:severity sh:Warning; #Mandatory if an equivalent scale or a resolution distance can be specified. Mandatory when there is a restriction on the spatial resolution for service.
  sh:datatype xsd:integer;
  sh:node inspire-shape:Integer;
  inspire-meta:isoref "60. equivalentScale";
  inspire-meta:xpath "identificationInfo[1]/*/spatialResolution/*/equivalentScale/*/denominator";
  skos:example "50000 (e.g. 1:50000 scale map)";
  rdfs:comment "For services, it is not possible to express the restriction of a service concerning the spatial resolution in the current version of ISO 19119. While the problem is addressed by the standardization community, spatial resolution restrictions for services shall be expressed in the Abstract";
.
inspire-shape:SpatialResolutionDistance a sh:PropertyShape;
  dct:subject inspire-concept:SpatialResolution;
  sh:name "spatialResolution";
  sh:severity sh:Warning; #Mandatory if an equivalent scale or a resolution distance can be specified. Mandatory when there is a restriction on the spatial resolution for service.
  sh:datatype xsd:decimal;
  sh:node inspire-shape:Distance;
  inspire-meta:isoref "61. distance";
  inspire-meta:xpath "identificationInfo[1]/*/spatialResolution/*/distance";
  skos:example "0.25 (degrees)";
  rdfs:comment "For services, it is not possible to express the restriction of a service concerning the spatial resolution in the current version of ISO 19119. While the problem is addressed by the standardization community, spatial resolution restrictions for services shall be expressed in the Abstract";
.
inspire-shape:Conformity a sh:PropertyShape;
  dct:subject inspire-concept:Conformity;
  sh:name "conformity";
  sh:severity sh:Violation;
  sh:node inspire-shape:ConformityElement;
  sh:nodeKind sh:BlankNode;
  sh:minCount 1;
  inspire-meta:xpath "dataQualityInfo/*/report/*/result/*/";
.
inspire-shape:ConformitySpecification a sh:PropertyShape;
  dct:subject inspire-concept:ConformitySpecification;
  sh:name "specification";
  sh:severity sh:Violation;
  sh:node inspire-shape:Citation; #359. CI_Citation
  sh:nodeKind sh:BlankNode;
  inspire-meta:isoref "130. specification";
  inspire-meta:xpath "dataQualityInfo/*/report/*/result/*/specification";
  skos:example '''- title: COMMISSION REGULATION (EU) No 1089/2010 of 23 November 2010 implementing Directive 2007/2/EC of the European Parliament and of the Council as regards interoperability of spatial data sets and services
- date:
  - dateType: publication
  - date: 2010-12-08'''
.
inspire-shape:ConformityDegree a sh:PropertyShape;
  dct:subject inspire-concept:ConformityDegree;
  sh:name "degree";
  sh:severity sh:Violation;
  sh:node inspire-shape:Boolean;
  sh:datatype xsd:boolean; #Datatype is specified as boolean, the legislation dictates a list of values (!) => D.5 is not used
  inspire-meta:isoref "132. pass";
  inspire-meta:xpath "dataQualityInfo/*/report/*/result/*/pass";
  skos:example "true";
  rdfs:comment '''- true if conformant
- false if not conformant
- null (with nilReason = 'unknown') if not evaluated'''
.
inspire-shape:ConditionsApplyingToAccessAndUse a sh:PropertyShape;
  dct:subject inspire-concept:ConditionsApplyingToAccessAndUse;
  sh:name "conditionsApplyingToAccessAndUse";
  sh:severity sh:Warning; #Mandatory if useConstraints is not documented.
  sh:class skos:Concept; #MD_RestrictionCode
  sh:node inspire-shape:AccessAndUseConditions; #Codelist (strictly limited to the value defined in B.5.24 of ISO 19115)
  inspire-meta:isoref "70. accessConstraints";
  inspire-meta:xpath "identificationInfo[1]/*/resourceConstraints/*/accessConstraints";
  skos:example "otherRestrictions (limitation not listed).";
.
inspire-shape:ConditionsApplyingToAccessAndUseOtherConstraints a sh:PropertyShape;
  dct:subject inspire-concept:ConditionsApplyingToAccessAndUse;
  sh:name "conditionsApplyingToAccessAndUse";
  sh:severity sh:Warning; #Mandatory if accessConstraints is set at the value "otherRestrictions"
  sh:node inspire-shape:FreeText;
  sh:datatype xsd:string; #CharacterString
  inspire-meta:isoref "72. otherConstraints";
  inspire-meta:xpath "identificationInfo[1]/*/resourceConstraints/*/otherConstraints";
  skos:example "http://inspire.ec.europa.eu/metadata-codelist/ConditionsApplyingToAccessAndUse/NoConditionsApply";
  skos:example "Reproduction for non-commercial purposes is authorised, provided the source is acknowledged. Commercial use is not permitted without prior written consent of the JRC. Reports, articles, papers, scientific and non-scientific works of any form, including tables, maps, or any other kind of output, in printed or electronic form, based in whole or in part on the data supplied, must contain an acknowledgement of the form: Data re-used from the European Drought Observatory (EDO) http://edo.jrc.ec.europa.eu The SPI data were created as part of JRC's research activities. Although every care has been taken in preparing and testing the data, JRC cannot guarantee that the data are correct; neither does JRC accept any liability whatsoever for any error, missing data or omission in the data, or for any loss or damage arising from its use. The JRC will not be responsible for any direct or indirect use which might be made of the data. The JRC does not provide any assistance or support in using the data";
  rdfs:comment '''The domain of the metadata element otherConstraints is Free text. This makes it hard to unambiguous define some common values in all official languages in the Communiy. Therefore it is required to refer to code lists in the Inspire registry for some specific values like "no conditions apply" and "conditions unknown" (see TG Requirement 8).'''
.
inspire-shape:ConditionsApplyingToUse a sh:Propertyshape;
  dct:subject inspire-concept:ConditionsApplyingToAccessAndUse;
  sh:name "conditionsApplyingToUse";
  sh:severity sh:Warning; #Mandatory if accessConstraints is not documented.
  sh:class skos:Concept; #MD_RestrictionCode
  sh:node inspire-shape:AccessAndUseConditions; #Codelist (strictly limited to the value defined in B.5.24 of ISO 19115)
  inspire-meta:isoref "71. useConstraints";
  inspire-meta:xpath "identificationInfo[1]/*/resourceConstraints/*/useConstraints";
  skos:example "otherRestrictions (limitation not listed).";
.
inspire-shape:ConditionsApplyingToUseOtherConstraints a sh:PropertyShape;
  dct:subject inspire-concept:ConditionsApplyingToAccessAndUse;
  sh:name "conditionsApplyingToUse";
  sh:severity sh:Warning; #Mandatory if useConstraints is set at the value "otherRestrictions"
  sh:node inspire-shape:FreeText;
  sh:datatype xsd:string; #CharacterString
  inspire-meta:isoref "72. otherConstraints";
  inspire-meta:xpath "identificationInfo[1]/*/resourceConstraints/*/otherConstraints";
  skos:example "http://inspire.ec.europa.eu/metadata-codelist/ConditionsApplyingToAccessAndUse/NoConditionsApply";
  skos:example "Reproduction for non-commercial purposes is authorised, provided the source is acknowledged. Commercial use is not permitted without prior written consent of the JRC. Reports, articles, papers, scientific and non-scientific works of any form, including tables, maps, or any other kind of output, in printed or electronic form, based in whole or in part on the data supplied, must contain an acknowledgement of the form: Data re-used from the European Drought Observatory (EDO) http://edo.jrc.ec.europa.eu The SPI data were created as part of JRC's research activities. Although every care has been taken in preparing and testing the data, JRC cannot guarantee that the data are correct; neither does JRC accept any liability whatsoever for any error, missing data or omission in the data, or for any loss or damage arising from its use. The JRC will not be responsible for any direct or indirect use which might be made of the data. The JRC does not provide any assistance or support in using the data";
  rdfs:comment '''The domain of the metadata element otherConstraints is Free text. This makes it hard to unambiguous define some common values in all official languages in the Communiy. Therefore it is required to refer to code lists in the Inspire registry for some specific values like "no conditions apply" and "conditions unknown" (see TG Requirement 8).'''
.
inspire-shape:LimitationsOnPublicAccess a sh:PropertyShape;
  dct:subject inspire-concept:LimitationsOnPublicAccess;
  sh:name "limitationsOnPublicAccess";
  sh:severity sh:Warning; #Mandatory if classification is not documented
  sh:class skos:Concept; #MD_RestrictionCode
  sh:node inspire-shape:AccessAndUseConditions; #Codelist (strictly limited to the value defined in B.5.24 of ISO 19115)
  sh:hasValue "otherConstraints";
  inspire-meta:isoref "70. accessConstraints";
  inspire-meta:xpath "identificationInfo[1]/*/resourceConstraints/*/accessConstraints";
  skos:example "otherRestrictions (limitation not listed).";
.
inspire-shape:LimitationsOnPublicAccessOtherConstraints a sh:PropertyShape;
  dct:subject inspire-concept:LimitationsOnPublicAccess;
  sh:name "limitationsOnPublicAccess";
  sh:severity sh:Warning; #Mandatory if classification is not documented
  sh:class skos:Concept; #Gmx:anchor
  sh:node inspire-shape:PublicAccessLimitations;
  inspire-meta:isoref "72. otherConstraints";
  inspire-meta:xpath "identificationInfo[1]/*/resourceConstraints/*/otherConstraints";
  skos:example '''<gmx:Anchor link:href=" http://inspire.ec.europa.eu/ metadata-codelist /LimitationsOnPublicAccess//NoLimitations"> no limitations</gmx:Anchor>''';
.
inspire-shape:ResponsibleOrganisation a sh:PropertyShape;
  dct:subject inspire-concept:ResponsibleOrganisation;
  inspire-meta:xpath "identificationInfo[1]/*/";
  sh:name "responsibleOrganisation";
  sh:minCount 1;
  sh:node inspire-shape:ResponsibleOrganisationElement;
  sh:nodeKind sh:BlankNode;
.
inspire-shape:ResponsibleParty a sh:PropertyShape;
  dct:subject inspire-concept:ResponsibleParty;
  sh:name "responsibleParty";
  sh:severity sh:Violation;
  sh:node inspire-shape:Party; #CI_ResponsibleParty
  sh:nodeKind sh:BlankNode;
  sh:minCount 1;
  sh:maxCount 1;
  inspire-meta:isoref "29. pointOfContact";
  inspire-meta:xpath "identificationInfo[1]/*/pointOfContact";
  skos:example '''- organisationName: European Commission, Joint Research Centre
- contactInfo:
  - address:
    - electronicMailAddress: ies-contact@jrc.ec.europa.eu'''
.
inspire-shape:ResponsibleOrganisationElement a sh:NodeShape;
  sh:name "+ResponsibleOrganisation";
  sh:property inspire-shape:ResponsibleParty;
  sh:property inspire-shape:ResponsiblePartyRole;
.
inspire-shape:Party a sh:NodeShape;
  dct:subject inspire-concept:Party;
  sh:name "+Party";
  sh:property [
    sh:name "organisationName";
    sh:datatype xsd:string;
    sh:node inspire-shape:FreeText
  ];
  sh:property [
    sh:name "contactInfo";
    sh:node inspire-shape:Contact;
  ];
.
inspire-shape:ResponsiblePartyRole a sh:PropertyShape;
  dct:subject inspire-concept:ResponsiblePartyRole;
  sh:name "responsiblePartyRole";
  sh:severity sh:Violation;
  sh:class skos:Concept; #CI_RoleCode
  sh:node inspire-shape:ResponsiblePartyRoles;
  sh:minCount 1;
  sh:maxCount 1;
  inspire-meta:isoref "379. role";
  inspire-meta:xpath "identificationInfo[1]/*/pointOfContact/*/role";
  skos:example "custodian";
  rdfs:comment "There is a direct mapping between the responsible party roles defined in Part D 6 of [Regulation 1205/2008] and the values of the CI_RoleCode code list of ISO 19115";
.
inspire-shape:MetadataPointOfContact a sh:PropertyShape;
  dct:subject inspire-concept:MetadataPointOfContact;
  sh:name "metadataPointOfContact";
  sh:severity sh:Violation;
  sh:node inspire-shape:Party; #CI_ResponsibleParty
  sh:nodeKind sh:BlankNode;
  sh:minCount 1;
  inspire-meta:isoref "8. contact";
  inspire-meta:xpath "contact";
  skos:example '''- organisationName: European Commission, Joint Research Centre
- contactInfo:
  - address:
  - electronicMailAddress: ies-contact@jrc.ec.europa.eu'''
.
inspire-shape:MetadataDate a sh:PropertyShape;
  dct:subject inspire-concept:MetadataDate;
  sh:name "date";
  sh:severity sh:Violation;
  sh:datatype xsd:date;
  sh:minCount 1;
  sh:maxCount 1;
  sh:node inspire-shape:Date;
  inspire-meta:isoref "9. dateStamp";
  inspire-meta:xpath "dateStamp";
  skos:example "2012-02-20";
.
inspire-shape:MetadataLanguage a sh:PropertyShape;
  dct:subject inspire-concept:MetadataLanguage;
  sh:name "language";
  sh:severity sh:Violation;
  sh:node inspire-shape:LanguageCode;
  sh:datatype xsd:string;
  inspire-meta:isoref "3. language";
  inspire-meta:xpath "language";
  skos:example "Eng";
.

#
# Section C.3 of Technical Guidance for the implementation of INSPIRE dataset and service metadata based on ISO/TS 19139:2007
#
inspire-shape:SpatialDatasetCoordinateReferenceSystem a sh:Propertyshape;
  dct:subject inspire-concept:SpatialDatasetCoordinateReferenceSystem;
  sh:name "coordinateReferenceSystem";
  sh:severity sh:Violation; #Mandatory for dataset and dataset series; not applicable to network services
  sh:minCount 1;
  sh:node inspire-shape:ReferenceSystem;
  sh:class inspire:CoordinateReferenceSystem;
  inspire-meta:isoref "13. referenceSystem";
  inspire-meta:xpath "referenceSystemInfo";
  skos:example "code: http://www.opengis.net/def/crs/EPSG/0/4258";
  rdfs:comment "ISO 19115 lists several elements which build MD_ReferenceSystem. For the purpose of theme-specific metadata according to the INSPIRE Data specifications the element listed above is sufficient."
.
inspire-shape:SpatialDatasetTemporalReferenceSystem a sh:PropertyShape;
  dct:subject inspire-concept:SpatialDatasetTemporalReferenceSystem;
  sh:name "temporal reference system";
  sh:severity sh:Warning; #Only required for dataset if non-default
  sh:node inspire-shape:ReferenceSystem;
  sh:class inspire:TemporalReferenceSystem;
  inspire-meta:isoref "13. referenceSystemInfo";
  inspire-meta:xpath "referenceSystemInfo";
  skos:example "JulianCalendar";
  rdfs:comment "The primary temporal reference system for use with geographic information is the Gregorian Calendar and 24 hour local or Coordinated Universal Time (UTC), but special applications may entail the use of alternative reference systems. So this element is mandatory only if the spatial data set contains temporal information that does not refer to the default temporal reference system.";
.
inspire-shape:SpatialDatasetEncoding a sh:PropertyShape;
  dct:subject inspire-concept:SpatialDatasetEncoding;
  sh:severity sh:Violation; #Only for dataset and dataset series
  sh:name "encoding";
  sh:minCount 1;
  sh:node inspire-shape:Format;
  sh:class inspire:Mediatype; #Not sure, could be something else!
  inspire-meta:isoref "271.distributionFormat";
  inspire-meta:xpath "distributionInfo/MD_Distribution/distributionFormat";
.
inspire-shape:SpatialDatasetCharacterEncoding a sh:PropertyShape;
  dct:subject inspire-concept:SpatialDatasetCharacterEncoding;
  sh:severity sh:Warning; # Mandatory if not UTF8. Not applicable to services
  sh:name "characterEncoding";
  sh:node inspire-shape:CharacterSet;
  sh:class inspire:CharacterSet;
  inspire-meta:isoref "40. characterSet";
  inspire-meta:xpath "identificationInfo[1]/*/characterSet";
  skos:example "usAscii";
.
inspire-shape:SpatialDatasetSpatialRepresentationType a sh:PropertyShape;
  dct:subject inspire-concept:SpatialDatasetSpatialRepresentationType;
  sh:severity sh:Violation; #Only for dataset and datasetseries, not applicable to services
  sh:name "spatialRepresentationType";
  sh:minCount 1;
  inspire-meta:isoref "37. SpatialRepresentationType";
  inspire-meta:xpath "identificationInfo[1]/*/spatialRepresentationType";
  sh:node inspire-shape:SpatialRepresentationTypeCode;
  sh:class skos:Concept;
  skos:example "vector";
  rdfs:comment "This element is used to broadly categorise a spatial data resource being described."
.
inspire-shape:SpatialDatasetTopologicalConsistencyQuantitive a sh:PropertyShape;
  dct:subject inspire-concept:SpatialDatasetTopologicalConsistency;
  sh:severity sh:Warning;
  sh:name "topologicalConsistency";
  sh:node inspire-shape:DataQualityElement;
  sh:nodeKind sh:BlankNode;
  inspire-meta:isoref "80. report";
  inspire-meta:xpath "dataQualityInfo/DQ_DataQuality/report/"
.
inspire-shape:SpatialDatasetTopologicalConsistencyDescriptive a sh:PropertyShape;
  dct:subject inspire-concept:SpatialDatasetTopologicalConsistency;
  sh:severity sh:Warning;
  sh:name "topologicalConsistency";
  sh:node inspire-shape:ConformanceResult;
  sh:nodeKind sh:BlankNode;
  inspire-meta:isoref "80. report";
  inspire-meta:xpath "dataQualityInfo/DQ_DataQuality/report/"
.  

#
# Section C.4 of Technical Guidance for the implementation of INSPIRE dataset and service metadata based on ISO/TS 19139:2007
#

inspire-shape:SpatialDataServicesCategory a sh:PropertyShape;
  dct:subject inspire-concept:SpatialDataServicesCategory;
  sh:name "category";
  inspire-meta:isoref "130. specification";
  inspire-meta:xpath "dataQualityInfo/*/report/*/result/*/specification";
  sh:severity sh:Violation; #Mandatory for invocable spatial data service
  sh:minCount 1;
  sh:maxCount 1;
  sh:node inspire-shape:SpatialDataServicesCategories;
  sh:class skos:Concept;
  skos:example '''<gmx:Anchor xlink:href=" http://inspire.ec.europa.eu/id/ats/metadata/2.0/sds-invocable" xlink:title="conformanceClass_Invocable">invocable</gmx:Anchor>'''
.

#
# Section C.5 of Technical Guidance for the implementation of INSPIRE dataset and service metadata based on ISO/TS 19139:2007
#

inspire-shape:CoordinateReferenceSystemIdentifier a sh:PropertyShape;
  dct:subject inspire-concept:CoordinateReferenceSystemIdentifier;
  sh:name "coordinateReferenceSystem";
  sh:node inspire-shape:ReferenceSystem;
  sh:class inspire:CoordinateReferenceSystem;
  inspire-meta:isoref "13. referenceSystem";
  inspire-meta:xpath "referenceSystemInfo";
  sh:severity sh:Violation; #Mandatory if relevant for interoperable spatial data services
.
inspire-shape:QualityOfService a sh:PropertyShape;
  dct:subject inspire-concept:QualityOfService;
  sh:name "qualityOfService";
  sh:node inspire-shape:QualityOfServiceElement;
  sh:nodeKind sh:BlankNode;
  sh:minCount 3;
  sh:maxCount 3;
  inspire-meta:xpath "dataQualityInfo/*/report/DQ_ConceptualConsistency/";
.
inspire-shape:QualityOfServiceCriteria a sh:PropertyShape;
  dct:subject inspire-concept:QualityOfServiceCriteria;
  sh:name "criteria";
  inspire-meta:isoref "100. nameOfMeasure";
  inspire-meta:xpath "dataQualityInfo/*/report/DQ_ConceptualConsistency/nameOfMeasure";
  sh:severity sh:Violation; #Mandatory for interoperable spatial data services
  sh:minCount 1;
  sh:maxCount 1;
  sh:node inspire-shape:QualityOfServiceCriteriaCodes;
  sh:class skos:Concept;
  skos:example "availability";
  rdfs:comment "The identifier of the measure is enough to retrieve all information about the quality measure. This element enable direct understanding of the metadata";
.
inspire-shape:QualityOfServiceMeasurementDescription a sh:PropertyShape;
  dct:subject inspire-concept:QualityOfServiceMeasurementDescription;
  sh:name "description";
  sh:severity sh:Violation; #Mandatory for interoperable spatial data services
  inspire-meta:isoref "101. measureIdentification";
  inspire-meta:xpath "dataQualityInfo/*/report/DQ_ConceptualConsistency/measureIdentification";
  sh:minCount 1;
  sh:maxCount 1;
  sh:datatype xsd:string; #Not sure
  sh:node inspire-shape:Code;
  skos:example "INSPIRE QoS2"
.
inspire-shape:QualityOfServiceMeasurementValue a sh:PropertyShape;
  dct:subject inspire-concept:QualityOfServiceMeasurementValue;
  sh:name "value";
  sh:severity sh:Violation; #Mandatory for interoperable spatial data services
  inspire-meta:isoref "137. value";
  inspire-meta:xpath "dataQualityInfo/*/report/DQ_ConceptualConsistency/result/DQ_QuantitativeResult/value";
  sh:minCount 1;
  sh:class rdfs:Literal;
  sh:node inspire-shape:ValueDatatype;
  skos:example "1";
.
inspire-shape:QualityOfServiceMeasurementUnit a sh:PropertyShape;
  dct:subject inspire-concept:QualityOfServiceMeasurementUnit;
  sh:name "unit";
  sh:severity sh:Violation; #Mandatory for interoperable spatial data services
  inspire-meta:isoref "135. valueUnit";
  inspire-meta:xpath "dataQualityInfo/*/report/DQ_ConceptualConsistency/result/DQ_QuantitativeResult/valueUnit";
  sh:node inspire-shape:UnitOfMeasure;
  sh:class inspire:UnitOfMeasure;
  sh:minCount 1;
  sh:maxCount 1;
  skos:example "second";
.
  
#
# Section C.6 of Technical Guidance for the implementation of INSPIRE dataset and service metadata based on ISO/TS 19139:2007
#
inspire-shape:OperationName a sh:PropertyShape;
  dct:subject inspire-concept:InvocationMetadata;
  sh:name "operationName";
  sh:severity sh:Violation; #Mandatory for harmonised spatial data services
  sh:minCount 1;
  sh:maxCount 1;
  sh:datatype xsd:string;
  sh:node inspire-shape:FreeText;
  inspire-meta:isoref "Table C2 1. operationName";
  inspire-meta:xpath "identificationInfo[1]/*/containsOperations/*/operationName";
  skos:example "GetSampleColumn";
.
inspire-shape:DCP a sh:PropertyShape;
  dct:subject inspire-concept:InvocationMetadata;
  sh:name "distributedComputingPlatform";
  sh:severity sh:Violation; #Mandatory for harmonised spatial data services
  sh:minCount 1;
  inspire-meta:isoref "Table C2 2. DCP";
  inspire-meta:xpath "identificationInfo[1]/*/containsOperations/*/DCP";
  sh:node inspire-shape:DCPList;
  sh:class skos:Concept;
  skos:example "WebServices";
.
inspire-shape:ConnectPoint a sh:PropertyShape;
  dct:subject inspire-concept:InvocationMetadata;
  sh:name "connectPoint";
  sh:severity sh:Violation; #Mandatory for harmonised spatial data services
  sh:minCount 1;
  sh:node inspire-shape:OnlineResource;
  sh:datatype xsd:anyURI;
  inspire-meta:isoref "Table C2 6. connectPoint";
  inspire-meta:xpath "identificationInfo[1]/*/containsOperations/*/connectPoint/*/linkage";
  skos:example "http://www.dinoservices.nl:80/geo3dmodelwebservices-1/Geo3DModelService";
.


#
# Section C.7 of Technical Guidance for the implementation of INSPIRE dataset and service metadata based on ISO/TS 19139:2007
#

# [This section is about specific extensions and not part of the core]

#
# Complex attributes
#
inspire-shape:ConformityElement a sh:NodeShape;
  sh:name "+Conformity";
  sh:property inspire-shape:ConformitySpecification;
  sh:property inspire-shape:ConformityDegree;
.
inspire-shape:Citation a sh:NodeShape;
  sh:name "+Citation";
  sh:property [
    sh:name "title";
    sh:datatype xsd:string;
    sh:node inspire-shape:FreeText;
    sh:minCount 1;
    sh:maxCount 1;
  ];
  sh:property [
    sh:name "referenceDate";
    sh:node inspire-shape:Date;
    sh:minCount 1;
    sh:maxCount 1;
    sh:nodeKind sh:BlankNode
  ];
.
inspire-shape:CIDate a sh:NodeShape;
  sh:name "+Date";
  sh:property [
    sh:name "dateType";
    sh:in ("creation" "publication" "revision");
    sh:datatype xsd:string;
    sh:minCount 1;
    sh:maxCount 1;
  ];
  sh:property [
    sh:name "date";
    sh:datatype xsd:date;
    sh:minCount 1;
    sh:maxCount 1;
  ]
.
inspire-shape:Period a sh:NodeShape;
  sh:name "+Period";
  sh:property [
    sh:name "begin";
    sh:datetype xsd:dateTime;
    sh:maxCount 1
  ];
  sh:property [
    sh:name "end";
    sh:datetype xsd:dateTime;
    sh:maxCount 1
  ]
.
inspire-shape:BoundingBox a sh:NodeShape;
  sh:name "+BoundingBox";
  sh:property [
    sh:name "westBoundLongitude";
    sh:datatype xsd:decimal;
    sh:minCount 1;
    sh:maxCount 1
  ];
  sh:property [
    sh:name "eastBoundLongitudeBoundLongitude";
    sh:datatype xsd:decimal;
    sh:minCount 1;
    sh:maxCount 1
  ];
  sh:property [
    sh:name "southBoundLatitudeBoundLatitude";
    sh:datatype xsd:decimal;
    sh:minCount 1;
    sh:maxCount 1
  ];
  sh:property [
    sh:name "northBoundLatitude";
    sh:datatype xsd:decimal;
    sh:minCount 1;
    sh:maxCount 1
  ];
.
inspire-shape:Format a sh:NodeShape;
  sh:name "*Format";
  sh:property [
    sh:name "name";
    sh:datatype xsd:string;
    sh:minCount 1;
    sh:maxCount 1
  ];
  sh:property [
    sh:name "version";
    sh:datatype xsd:string;
    sh:minCount 1;
    sh:maxCount 1
  ]
.
inspire-shape:DataQualityElement a sh:NodeShape;
  sh:name "+DataQualityElement";
  sh:property [
    sh:name "nameOfMeasure";
  ];
  sh:property [
    sh:name "evaluationMethodType";
    sh:maxCount 1;
  ];
  sh:property [
    sh:name "evaluationMethodDescription";
    sh:maxCount 1;
  ];
  sh:property [
    sh:name "dateTime";
  ];
  sh:property [
    sh:name "result";
    sh:minCount 1;
    sh:maxCount 2;
  ];
.
inspire-shape:QualityOfServiceElement a sh:NodeShape;
  sh:name "+QualityOfService";
  sh:property inspire-shape:QualityOfServiceCriteria;
  sh:property inspire-shape:QualityOfServiceMeasurementDescription;
  sh:property inspire-shape:QualityOfServiceMeasurementUnit;
  sh:property inspire-shape:QualityOfServiceMeasurementValue;
.
inspire-shape:ConformanceResult a sh:NodeShape;
  sh:name "+ConformanceResult";
  sh:property [
    sh:name "specification";
    sh:minCount 1;
    sh:maxCount 1;
    sh:node inspire-shape:Citation;
    sh:nodeKind sh:BlankNode;
  ];
  sh:property [
    sh:name "explanation";
    sh:minCount 1;
    sh:maxCount 1;
  ];
  sh:property [
    sh:name "pass";
    sh:minCount 1;
    sh:maxCount 1;
    sh:datatype xsd:boolean;
  ];
.
inspire-shape:ResourceLocatorElement a sh:NodeShape;
  sh:name "+ResourceLocatorElement";
  sh:property [
    sh:name "URL";
    sh:datatype xsd:AnyURI;
  ];
  sh:property [
    sh:name "title";
    sh:datatype xsd:string;
  ];
  sh:property [
    sh:name "name";
    sh:datatype xsd:string; #Not quite sure if it should be "name" or "title". Both are mentioned
  ];
  sh:property [
    sh:name "description";
    sh:datatype xsd:string;
  ];
  sh:property [
    sh:name "description";
    sh:node inspire-shape:OnlineDescriptionCodes;
  ];
  sh:property [
    sh:name "function";
    sh:node inspire-shape:OnlineFunctionCodes;
  ]
.
inspire-shape:Contact a sh:NodeShape;
  sh:name "+Contact";
  sh:property [
    sh:name "address";
    sh:node inspire-shape:Address;
    sh:nodeKind sh:BlankNode;
  ]
.
inspire-shape:Address a sh:NodeShape;
  sh:name "+Address";
  sh:property [
    sh:name "electronicMailAddress";
    sh:minCount 1;
    sh:datatype xsd:string;
  ];
.
inspire-shape:ReferenceSystem a sh:NodeShape;
  sh:name "*ReferenceSystem";
  sh:property [
    sh:name "code";
    sh:datatype xsd:string;
    sh:minCount 1;
    sh:maxCount 1;
  ];
  sh:property [
    sh:name "description";
    sh:datatype xsd:string;
    sh:minCount 1;
    sh:maxCount 1;
  ];
.
inspire-shape:KeywordElement a sh:NodeShape;
  sh:name "+Keyword";
  sh:property inspire-shape:KeywordValue;
  sh:property inspire-shape:KeywordOriginatingControlledVocabulary;
.

#
# Domain: Data types
#
inspire-shape:FreeText a sh:Nodeshape;
  sh:name "*Free text";
.
inspire-shape:OnlineResource a sh:NodeShape;
  sh:name "*Online resource";
.
inspire-shape:ValueDatatype a sh:NodeShape;
  sh:name "*ValueDatatype";
  rdfs:comment "Any datatype according to the specific measurement";
.
inspire-shape:Code a sh:Nodeshape;
  sh:name "*Code";
  rdfs:comment "Some code identifier. In case a predefined list is not available (in such cases, codes would be part of a skos:notation element)";
.
inspire-shape:UnitOfMeasure a sh:NodeShape;
  sh:name "*UnitOfMeasure";
.
inspire-shape:Mediatype a sh:NodeShape;
  sh:name "*Mediatype";
.
inspire-shape:CharacterSet a sh:NodeShape;
  sh:name "*CharacterSet";
.
inspire-shape:URL a sh:NodeShape;
  sh:name "*URL";
.
inspire-shape:URI a sh:NodeShape;
  sh:name "*URI";
.
inspire-shape:LanguageCode a sh:NodeShape;
  sh:name "*LanguageCode";
.
inspire-shape:Integer a sh:NodeShape;
  sh:name "*Integer";
.
inspire-shape:Distance a sh:NodeShape;
  sh:name "*Distance";
.
inspire-shape:Boolean a sh:NodeShape;
  sh:name "*Boolean";
.
inspire-shape:Date a sh:NodeShape;
  sh:name "*Date";
.

#
# Waardelijsten
#
inspire-shape:ResourceTypes a sh:NodeShape;
  sh:name "CodeList (see annex B.5.25 of ISO 19115)";
  sh:property [
    sh:path [sh:inversePath skos:member];
    sh:hasValue inspire-collection:ResourceTypes
  ]
.
inspire-shape:TopicCategories a sh:NodeShape;
  sh:name "Enumeration (See B.5.27 of ISO 19115 or Part D 2 of [Regulation 1205/2008])";
  sh:property [
    sh:path [sh:inversePath skos:member];
    sh:hasValue inspire-collection:TopicCategories
  ]
.
inspire-shape:SpatialDataServiceTypes a sh:NodeShape;
  sh:name "Code list. See Part D 3 of [Regulation 1205/2008]";
  sh:property [
    sh:path [sh:inversePath skos:member];
    sh:hasValue inspire-collection:SpatialDataServiceTypes
  ]
.
inspire-shape:AccessAndUseConditions a sh:NodeShape;
  sh:name "Codelist (strictly limited to the value defined in B.5.24 of ISO 19115)";
  sh:property [
    sh:path [sh:inversePath skos:member];
    sh:hasValue inspire-collection:AccessAndUseConditions
  ]
.
inspire-shape:PublicAccessLimitations a sh:NodeShape;
  sh:name "Anex D.1 Limitations on public access";
  sh:property [
    sh:path [sh:inversePath skos:member];
    sh:hasValue inspire-collection:PublicAccessLimitations
  ]
.
inspire-shape:ResponsiblePartyRoles a sh:NodeShape;
  sh:name "Codelist (see B.5.5 of ISO 19115)";
  sh:property [
    sh:path [sh:inversePath skos:member];
    sh:hasValue inspire-collection:ResponsiblePartyRoles
  ]
.
inspire-shape:SpatialDataServicesCategories a sh:NodeShape;
  sh:name "Enumeration (invocable, interoperable, harmonized)";
  sh:property [
    sh:path [sh:inversePath skos:member];
    sh:hasValue inspire-collection:SpatialDataServicesCategories
  ]
.
inspire-shape:QualityOfServiceCriteriaCodes a sh:NodeShape;
  sh:name "Enumeration (availability, performance, capacity)";
  sh:property [
    sh:path [sh:inversePath skos:member];
    sh:hasValue inspire-collection:QualityOfServiceCriteriaCodes
  ]
.
inspire-shape:OnlineFunctionCodes a sh:NodeShape;
  sh:name "OnlineFunctionCodes";
  sh:property [
    sh:path [sh:inversePath skos:member];
    sh:hasValue inspire-collection:OnlineFunctionCodes
  ]
.
inspire-shape:OnlineDescriptionCodes a sh:NodeShape;
  sh:name "OnlineDescriptionCodes";
  sh:property [
    sh:path [sh:inversePath skos:member];
    sh:hasValue inspire-collection:OnlineDescriptionCodes
  ]
.
inspire-shape:DCPList a sh:NodeShape;
  sh:name "DCPList";
  sh:property [
    sh:path [sh:inversePath skos:member];
    sh:hasValue inspire-collection:DCPList
  ]
.
inspire-shape:SpatialRepresentationTypeCode a sh:NodeShape;
  sh:name "SpatialRepresentationTypeCode";
  sh:property [
    sh:path [sh:inversePath skos:member];
    sh:hasValue inspire-collection:SpatialRepresentationTypeCode
  ]
.

#
# Technische waardelijsten
#
inspire-collection:PublicAccessLimitations a skos:Collection;
  rdfs:label "Limitations on public access";
  skos:member inspire-concept:NoLimitations;
  skos:member inspire-concept:INSPIRE_Directive_Article13_1a;
  skos:member inspire-concept:INSPIRE_Directive_Article13_1b;
  skos:member inspire-concept:INSPIRE_Directive_Article13_1c;
  skos:member inspire-concept:INSPIRE_Directive_Article13_1d;
  skos:member inspire-concept:INSPIRE_Directive_Article13_1e;
  skos:member inspire-concept:INSPIRE_Directive_Article13_1f;
  skos:member inspire-concept:INSPIRE_Directive_Article13_1g;
  skos:member inspire-concept:INSPIRE_Directive_Article13_1h;
.
inspire-concept:NoLimitations a skos:Concept;
  rdfs:label "No limitations to public access";
  skos:definition "There are no limitations on public access to spatial data sets and services";
  skos:notation "noLimitations";
.
inspire-concept:INSPIRE_Directive_Article13_1a a skos:Concept;
  dct:source inspire-lex:Article13-1-a;
  rdfs:label "public access limited according to Article 13(1)(a) of the INSPIRE Directive";
  skos:definition "Public access to spatial data sets and services would adversely affect the confidentiality of the proceedings of public authorities, where such confidentiality is provided for by law.";
  skos:notation "INSPIRE_Directive_Article13_1a"
.

inspire-collection:OnlineFunctionCodes a skos:Collection;
  rdfs:label "Online function codes";
  skos:member inspire-concept:Download;
  skos:member inspire-concept:Information;
  skos:member inspire-concept:OfflineAccess;
  skos:member inspire-concept:Order;
  skos:member inspire-concept:Search;
.
inspire-concept:Download a skos:Concept;
  rdfs:label "Download"@en;
  skos:definition "online instructions for transferring data from one storage device or system to another"@en;
.
inspire-concept:Information a skos:Concept;
  rdfs:label "Information"@en;
  skos:definition "online information about the resource";
.
inspire-concept:OfflineAccess a skos:Concept;
  rdfs:label "Offline access"@en;
  skos:definition "online instructions for requesting the resource from the provider"@en;
.
inspire-concept:Order a skos:Concept;
  rdfs:label "Order"@en;
  skos:definition "online order process for obtening the resource"@en;
.
inspire-concept:Search a skos:Concept;
  rdfs:label "Search"@en;
  skos:definition "online search interface for seeking out information about the resource"@en;
.

inspire-collection:OnlineDescriptionCodes a skos:Collection;
  rdfs:label "Online description codes";
  skos:member inspire-concept:AccessPoint;
  skos:member inspire-concept:EndPoint;
.

inspire-collection:DCPList a skos:Collection;
  rdfs:label "Distributed Computing Platforms";
  skos:member inspire-concept:XML;
  skos:member inspire-concept:CORBA;
  skos:member inspire-concept:JAVA;
  skos:member inspire-concept:COM;
  skos:member inspire-concept:SQL;
  skos:member inspire-concept:WebServices;
.
inspire-concept:XML a skos:Concept;
  rdfs:label "XML";
.
inspire-concept:CORBA a skos:Concept;
  rdfs:label "CORBA";
.
inspire-concept:JAVA a skos:Concept;
  rdfs:label "JAVA";
.
inspire-concept:COM a skos:Concept;
  rdfs:label "COM";
.
inspire-concept:SQL a skos:Concept;
  rdfs:label "SQL";
.
inspire-concept:WebServices a skos:Concept;
  rdfs:label "WebServices";
.

inspire-collection:SpatialRepresentationTypeCode a skos:Collection;
  rdfs:label "Spatial representation type codes";
  skos:member inspire-concept:Vector;
  skos:member inspire-concept:Grid;
  skos:member inspire-concept:Tin;
.